union_inc_iff

Matroid/Graph/Operations/Union.lean
@@ -626,13 +626,13 @@ protected def union (G H : Graph α β) : Graph α β where
     refine ⟨fun he => ?_, by rintro ⟨x, y, u, v, (hl | ⟨hl, -⟩), hxu, hyv⟩ <;> simp [hl.edge_mem]⟩
     by_cases heG : e ∈ E(G)
     · obtain ⟨x, y, hl⟩ := exists_isLink_of_mem_edgeSet heG
-      use x, y, x, y, Or.inl hl, ?_ <;> rw [Relation.transGen_self_iff] <;> left
-      · exact G.dup_refl_iff.mp hl.right_mem
-      exact G.dup_refl_iff.mp hl.left_mem
+      use x, y, x, y, Or.inl hl, ?_ <;> rw [← union_dup_refl_iff] <;> left
+      · exact hl.right_mem
+      exact hl.left_mem
     · obtain ⟨x, y, hl⟩ := exists_isLink_of_mem_edgeSet <| he.resolve_left heG
-      use x, y, x, y, Or.inr ⟨hl, heG⟩, ?_ <;> rw [Relation.transGen_self_iff] <;> right
-      · exact H.dup_refl_iff.mp hl.right_mem
-      exact H.dup_refl_iff.mp hl.left_mem
+      use x, y, x, y, Or.inr ⟨hl, heG⟩, ?_ <;> rw [← union_dup_refl_iff] <;> right
+      · exact hl.right_mem
+      exact hl.left_mem
 
 instance : Union (Graph α β) where union := Graph.union
 
@@ -642,900 +642,910 @@ lemma union_vertexSet (G H : Graph α β) : V(G ∪ H) = V(G) ∪ V(H) := rfl
 @[simp]
 lemma union_edgeSet (G H : Graph α β) : E(G ∪ H) = E(G) ∪ E(H) := rfl
 
-lemma union_eq_sUnion (G H : Graph α β) : G ∪ H = Graph.sUnion {G, H ＼ E(G)} (by simp) := by
-  simp_rw [Union.union, Graph.union, Graph.copy]
-  ext <;> simp
-
-lemma union_isLink_iff :
-    (G ∪ H).IsLink e x y ↔ G.IsLink e x y ∨ (H.IsLink e x y ∧ e ∉ E(G)) := by
-  simp [union_eq_sUnion]
-
-lemma union_inc_iff : (G ∪ H).Inc e x ↔ G.Inc e x ∨ (H.Inc e x ∧ e ∉ E(G)) := by
-  simp [union_eq_sUnion]
-
-lemma union_isLoopAt_iff : (G ∪ H).IsLoopAt e x ↔ G.IsLoopAt e x ∨ (H.IsLoopAt e x ∧ e ∉ E(G)) := by
-  simp [union_eq_sUnion]
-
-lemma union_isNonloopAt_iff :
-    (G ∪ H).IsNonloopAt e x ↔ G.IsNonloopAt e x ∨ (H.IsNonloopAt e x ∧ e ∉ E(G)) := by
-  simp only [IsNonloopAt, ne_eq, union_isLink_iff]
-  aesop
-
-lemma union_eq_union_edgeDelete (G H : Graph α β) : G ∪ H = G ∪ (H ＼ E(G)) := by
-  simp [union_eq_sUnion, union_eq_sUnion]
+@[simp]
+lemma union_dup : (G ∪ H).dup x y ↔ Relation.TransGen (G.dup ⊔ H.dup) x y := Iff.rfl
 
 @[simp]
-protected lemma left_le_union (G H : Graph α β) : G ≤ G ∪ H := by
-  simp_rw [le_iff, union_isLink_iff]
-  tauto
-
-protected lemma union_le {H₁ H₂ : Graph α β} (h₁ : H₁ ≤ G) (h₂ : H₂ ≤ G) : H₁ ∪ H₂ ≤ G := by
-  simp [union_eq_sUnion, h₁, edgeDelete_le.trans h₂]
-
-lemma union_le_iff {H₁ H₂ : Graph α β} : H₁ ∪ H₂ ≤ G ↔ H₁ ≤ G ∧ H₂ ＼ E(H₁) ≤ G := by
-  simp [union_eq_sUnion]
-
-lemma union_mono_right (h : H₁ ≤ H₂) : G ∪ H₁ ≤ G ∪ H₂ := by
-  simp only [union_eq_sUnion, Graph.sUnion_le_iff, mem_insert_iff, mem_singleton_iff,
-    forall_eq_or_imp, forall_eq]
-  exact ⟨Graph.le_sUnion _ (by simp), le_trans (edgeDelete_mono_left h) <|
-    Graph.le_sUnion _ (by simp : H₂ ＼ E(G) ∈ _)⟩
+lemma union_isLink : (G ∪ H).IsLink e x y ↔
+    ∃ u v, (G.IsLink e u v ∨ (H.IsLink e u v ∧ e ∉ E(G))) ∧
+    Relation.TransGen (G.dup ⊔ H.dup) x u ∧ Relation.TransGen (G.dup ⊔ H.dup) y v := Iff.rfl
 
 @[simp]
-protected lemma union_self (G : Graph α β) : G ∪ G = G :=
-  (Graph.union_le le_rfl le_rfl).antisymm <| Graph.left_le_union ..
-
-protected lemma union_assoc (G₁ G₂ G₃ : Graph α β) : (G₁ ∪ G₂) ∪ G₃ = G₁ ∪ (G₂ ∪ G₃) := by
-  refine Graph.ext (Set.union_assoc ..) fun e x y ↦ ?_
-  simp [union_isLink_iff]
-  tauto
-
-lemma isLink_or_isLink_of_union (h : (G ∪ H).IsLink e x y) : G.IsLink e x y ∨ H.IsLink e x y :=
-  (union_isLink_iff.1 h).elim .inl fun h' ↦ .inr h'.1
-
-lemma Compatible.union_isLink_iff (h : G.Compatible H) :
-    (G ∪ H).IsLink e x y ↔ G.IsLink e x y ∨ H.IsLink e x y := by
-  by_cases heG : e ∈ E(G)
-  · simp only [Graph.union_isLink_iff, heG, not_true_eq_false, and_false, or_false, iff_self_or]
-    exact fun he ↦ by rwa [h.isLink_eq heG he.edge_mem]
-  simp [heG, Graph.union_isLink_iff]
-
-lemma edgeRestrict_union (G : Graph α β) (F₁ F₂ : Set β) : (G ↾ (F₁ ∪ F₂)) = G ↾ F₁ ∪ (G ↾ F₂) := by
-  refine Graph.ext (by simp) fun e x y ↦ ?_
-  rw [(G.compatible_self.mono (by simp) (by simp)).union_isLink_iff]
-  simp only [edgeRestrict_isLink, mem_union]
-  tauto
-
-lemma Compatible.union_eq_sUnion (h : G.Compatible H) :
-    G ∪ H = Graph.sUnion {G, H} (by simp [Set.pairwise_iff_of_refl, h, h.symm]) :=
-  Graph.ext (by simp) fun e x y ↦ by simp [h.union_isLink_iff]
-
-lemma Compatible.union_inc_iff (h : G.Compatible H) : (G ∪ H).Inc e x ↔ G.Inc e x ∨ H.Inc e x := by
-  simp_rw [Inc, h.union_isLink_iff]
-  aesop
-
-lemma Compatible.union_isLoopAt_iff (h : G.Compatible H) :
-    (G ∪ H).IsLoopAt e x ↔ G.IsLoopAt e x ∨ H.IsLoopAt e x := by
-  simp_rw [← isLink_self_iff, h.union_isLink_iff]
-
-lemma Compatible.union_isNonloopAt_iff (h : G.Compatible H) :
-    (G ∪ H).IsNonloopAt e x ↔ G.IsNonloopAt e x ∨ H.IsNonloopAt e x := by
-  simp_rw [IsNonloopAt, h.union_isLink_iff]
-  aesop
-
-lemma Compatible.union_adj_iff (h : G.Compatible H) : (G ∪ H).Adj x y ↔ G.Adj x y ∨ H.Adj x y := by
-  simp [Adj, h.union_isLink_iff, exists_or]
-
-lemma Compatible.union_comm (h : Compatible G H) : G ∪ H = H ∪ G :=
-  Graph.ext (Set.union_comm ..)
-    fun _ _ _ ↦ by rw [h.union_isLink_iff, h.symm.union_isLink_iff, or_comm]
-
-lemma Compatible.union_le_iff {H₁ H₂ : Graph α β} (h_compat : H₁.Compatible H₂) :
-    H₁ ∪ H₂ ≤ G ↔ H₁ ≤ G ∧ H₂ ≤ G := by
-  simp [h_compat.union_eq_sUnion]
-
-lemma Compatible.right_le_union (h : G.Compatible H) : H ≤ G ∪ H := by
-  simp [h.union_comm]
-
-lemma union_eq_self_of_le_left (hle : G ≤ H) : G ∪ H = H :=
-  (Graph.union_le hle rfl.le).antisymm (H.compatible_self.mono_left hle).right_le_union
-
-lemma union_eq_self_of_le_right (hle : G ≤ H) : H ∪ G = H :=
-  (Graph.union_le rfl.le hle).antisymm <| Graph.left_le_union ..
-
-lemma Compatible.union_mono_left (h : H₂.Compatible G) (hle : H₁ ≤ H₂) : H₁ ∪ G ≤ H₂ ∪ G := by
-  rw [h.union_comm, (h.mono_left hle).union_comm]
-  exact union_mono_right hle
-
-lemma Compatible.union_mono (hleG : G₁ ≤ G₂) (hleH : H₁ ≤ H₂) (h : G₂.Compatible H₁) :
-    G₁ ∪ H₁ ≤ G₂ ∪ H₂ := le_trans (h.union_mono_left hleG) (union_mono_right hleH)
-
-lemma edgeRestrict_union_edgeDelete (G : Graph α β) (F : Set β) : (G ↾ F) ∪ (G ＼ F) = G := by
-  rw [edgeDelete_eq_edgeRestrict, ← edgeRestrict_union, ← edgeRestrict_inter_edgeSet]
-  simp only [union_diff_self, edgeRestrict_inter_edgeSet, edgeRestrict_union, edgeRestrict_self]
-  exact union_eq_self_of_le_left (by simp)
-
-lemma edgeDelete_union_edgeRestrict (G : Graph α β) (F : Set β) : (G ＼ F) ∪ (G ↾ F) = G := by
-  convert G.edgeRestrict_union_edgeDelete F using 1
-  rw [Compatible.union_comm]
-  apply G.compatible_of_le_le (by simp) (by simp)
-
-lemma induce_union_edgeDelete (G : Graph α β) (hX : X ⊆ V(G)) : G[X] ∪ (G ＼ E(G[X])) = G := by
-  rw [← union_eq_union_edgeDelete, union_eq_self_of_le_left (induce_le hX)]
-
-lemma edgeDelete_union_induce (G : Graph α β) (hX : X ⊆ V(G)) : (G ＼ E(G[X])) ∪ G[X] = G := by
-  rw [(Compatible.of_disjoint_edgeSet _).union_comm, induce_union_edgeDelete _ hX]
-  simp [disjoint_sdiff_left]
-
-lemma Compatible.union_eq_iUnion (h : G.Compatible H) :
-    G ∪ H = Graph.iUnion (fun b ↦ bif b then G else H) (by simpa [pairwise_on_bool]) := by
-  generalize_proofs h'
-  simp only [le_antisymm_iff, h.union_le_iff, Graph.iUnion_le_iff, Bool.forall_bool, cond_false,
-    h.right_le_union, cond_true, Graph.left_le_union, and_self, and_true]
-  exact ⟨Graph.le_iUnion h' true, Graph.le_iUnion h' false⟩
-
-lemma Compatible.induce_union (h : G.Compatible H) (X : Set α) : (G ∪ H)[X] = G[X] ∪ H[X] := by
-  refine Graph.ext (by simp) fun e x y ↦ ?_
-  simp only [induce_isLink_iff, h.union_isLink_iff, h.induce.union_isLink_iff]
-  tauto
-
-lemma Compatible.vertexDelete_union (h : G.Compatible H) (X : Set α) :
-    (G ∪ H) - X = (G - X) ∪ (H - X) := by
-  simp only [h.union_eq_iUnion, vertexDelete_iUnion, Bool.apply_cond (f := fun G ↦ G - X),
-    ← h.vertexDelete.union_eq_iUnion]
-
-lemma induce_union (G : Graph α β) (X Y : Set α) (hX : ∀ x ∈ X, ∀ y ∈ Y, ¬ G.Adj x y) :
-    G [X ∪ Y] = G [X] ∪ G [Y] := by
-  refine Graph.ext rfl fun e x y ↦ ?_
-  simp only [induce_isLink_iff, mem_union, Compatible.induce_induce.union_isLink_iff]
-  by_cases hxy : G.IsLink e x y
-  · by_cases hx : x ∈ X
-    · simp [hx, show y ∉ Y from fun hy ↦ hX x hx y hy hxy.adj]
-    by_cases hy : y ∈ X
-    · simp [hy, show x ∉ Y from fun hx ↦ hX _ hy _ hx hxy.symm.adj, hxy]
-    simp [hx, hy]
-  simp [hxy]
-
-/-! ### Indexed Intersections -/
-
-/-- The intersection of a nonempty family of pairwise compatible graphs.
-  Remove any disagreeing edges. -/
-@[simps]
-protected def iInter [Nonempty ι] (G : ι → Graph α β) : Graph α β where
-  vertexSet := ⋂ i, V(G i)
-  dup x y := ∀ i, (G i).dup x y
-  dup_refl_iff x := by simp [dup_refl_iff]
-  dup_symm := by
-    simp_rw [dup_comm]
-    exact fun _ _ a ↦ a
-  dup_trans x y z hxy hyz i := (hxy i).trans (hyz i)
-  edgeSet := {e | ∃ x y, ∀ i, (G i).IsLink e x y}
-  IsLink e x y := ∀ i, (G i).IsLink e x y
-  isLink_symm e he x y := by simp [isLink_comm]
-  dup_or_dup_of_isLink_of_isLink e u v x y h h' := by
-    let i' := Classical.arbitrary ι
-    obtain hux | huy := dup_or_dup_of_isLink_of_isLink _ (h i') (h' i')
-    · sorry
-    sorry
-  edge_mem_iff_exists_isLink e := by simp
-  left_mem_of_isLink e x y h := mem_iInter.2 fun i ↦ (h i).left_mem
-  isLink_of_dup e x y z hxy hxz i := (hxy i |>.symm.isLink_left).mpr <| hxz i
-
-protected lemma iInter_le {G : ι → Graph α β} [Nonempty ι] (i : ι) : Graph.iInter G ≤ G i where
-  vertex_subset := iInter_subset (fun i ↦ V(G i)) i
-  isLink_of_isLink _ _ _ h := h i
-
-@[simp]
-lemma le_iInter_iff [Nonempty ι] {G : ι → Graph α β} :
-    H ≤ Graph.iInter G ↔ ∀ i, H ≤ G i := by
-  let j := Classical.arbitrary ι
-  refine ⟨fun h i ↦ h.trans <| Graph.iInter_le .., fun h ↦ ?_⟩
-  apply le_of_le_le_subset_subset (h j) (Graph.iInter_le ..) ?_ fun e he ↦ ?_
-  · simp [fun i ↦ vertexSet_mono (h i)]
-  simp only [iInter_edgeSet, mem_setOf_eq]
-  obtain ⟨x, y, hbtw⟩ := exists_isLink_of_mem_edgeSet he
-  use x, y, fun i ↦ hbtw.of_le (h i)
-
-@[simp]
-protected lemma iInter_const [Nonempty ι] (G : Graph α β) :
-    Graph.iInter (fun (_ : ι) ↦ G) = G := by
-  apply le_antisymm (Graph.iInter_le (Classical.arbitrary ι))
-  rw [le_iInter_iff]
-  exact fun i ↦ le_refl G
-
-lemma iInter_le_iUnion [Nonempty ι] {G : ι → Graph α β} (hG : Pairwise (Compatible on G)) :
-    Graph.iInter G ≤ Graph.iUnion G hG :=
-  (Graph.iInter_le (Classical.arbitrary ι)).trans <| Graph.le_iUnion ..
-
-protected lemma iInter_comp_le [Nonempty ι] [Nonempty ι'] {f : ι' → ι}
-    {G : ι → Graph α β} : Graph.iInter G ≤ Graph.iInter (fun i ↦ G (f i)) := by
-  rw [Graph.le_iInter_iff]
-  exact fun i ↦ Graph.iInter_le (f i)
-
-lemma iInter_comp_eq_of_surj [Nonempty ι] [Nonempty ι'] {f : ι' → ι}
-    {G : ι → Graph α β} (hf : Function.Surjective f) :
-    Graph.iInter G = Graph.iInter (fun i ↦ G (f i)) :=
-  le_antisymm (Graph.iInter_comp_le) <| by
-  rw [Graph.le_iInter_iff]
-  rintro i
-  obtain ⟨i', rfl⟩ := hf i
-  exact Graph.iInter_le i'
-
-lemma iInter_range [Nonempty ι'] {f : ι' → ι} {G : (Set.range f) → Graph α β} :
-    Graph.iInter G = Graph.iInter (fun i ↦ G (Set.rangeFactorization f i)) :=
-  iInter_comp_eq_of_surj surjective_onto_range
-
-@[simp]
-lemma iInter_inc_iff [Nonempty ι] {G : ι → Graph α β} :
-    (Graph.iInter G).Inc e x ↔ ∃ y, ∀ i, (G i).IsLink e x y := by
-  simp only [Inc, iInter_isLink]
-
-@[simp]
-lemma iInter_isLoopAt_iff [Nonempty ι] {G : ι → Graph α β} :
-    (Graph.iInter G).IsLoopAt e x ↔ ∀ i, (G i).IsLoopAt e x := by
-  simp only [IsLoopAt, iInter_isLink]
-
-@[simp]
-lemma iInter_isNonloopAt_iff [Nonempty ι] {G : ι → Graph α β} :
-    (Graph.iInter G).IsNonloopAt e x ↔ ∃ y ≠ x, ∀ i, (G i).IsLink e x y := by
-  simp only [IsNonloopAt, iInter_isLink]
-
-@[simp]
-lemma induce_iInter [Nonempty ι] {G : ι → Graph α β} (X : Set α) :
-    (Graph.iInter G)[X] = .iInter (fun i ↦ (G i)[X]) :=
-  Graph.ext (iInter_const X).symm fun e x y ↦ by
-  simp [forall_and_right]
-
-@[simp]
-lemma vertexDelete_iInter [Nonempty ι] {G : ι → Graph α β} (X : Set α) :
-    (Graph.iInter G) - X = .iInter (fun i ↦ (G i) - X) :=
-  Graph.ext (by simp) fun e x y ↦ by
-  simp +contextual only [vertexDelete_isLink_iff, iInter_isLink, iff_def, not_false_eq_true,
-    and_self, implies_true, true_and]
-  exact fun h ↦ (h <| Classical.arbitrary ι).right
-
-@[simp]
-lemma edgeDelete_iInter [Nonempty ι] {G : ι → Graph α β} (F : Set β) :
-    (Graph.iInter G) ＼ F = .iInter (fun i ↦ (G i) ＼ F) :=
-  Graph.ext (by simp) fun e x y ↦ by
-  simp +contextual only [edgeDelete_isLink, iInter_isLink, iff_def, not_false_eq_true, and_self,
-    implies_true, true_and]
-  exact fun h ↦ (h <| Classical.arbitrary ι).right
-
-@[simp]
-lemma edgeRestrict_iInter [Nonempty ι] {G : ι → Graph α β} (F : Set β) :
-    (Graph.iInter G) ↾ F = .iInter (fun i ↦ (G i) ↾ F) :=
-  Graph.ext (by simp) fun e x y ↦ by
-  simp +contextual only [edgeRestrict_isLink, iInter_isLink, iff_def, and_self, implies_true,
-    and_true, true_and]
-  exact fun h ↦ (h <| Classical.arbitrary ι).left
-
-/-! ### Set Intersections -/
-
-/-- The intersection of a nonempty set of pairwise compatible graphs. -/
-@[simps!]
-protected def sInter (s : Set (Graph α β)) (hne : s.Nonempty) :
-    Graph α β :=
-  @Graph.iInter _ _ _ hne.to_subtype (fun G : s ↦ G.1)
-
-protected lemma sInter_le {s : Set (Graph α β)} (hG : G ∈ s) :
-    Graph.sInter s ⟨G, hG⟩ ≤ G := by
-  rw [Graph.sInter]
-  generalize_proofs h
-  exact Graph.iInter_le (⟨G, hG⟩ : s)
-
-@[simp]
-protected lemma le_sInter_iff {s} (hne : s.Nonempty) :
-    H ≤ Graph.sInter s hne ↔ ∀ G ∈ s, H ≤ G := by
-  simp [Graph.sInter]
-
-protected lemma sInter_anti {s t : Set (Graph α β)} (hne : s.Nonempty) (hne' : t.Nonempty)
-    (hle : s ⊆ t) : Graph.sInter t hne' ≤ Graph.sInter s hne := by
-  rw [Graph.le_sInter_iff hne]
-  exact fun G hGs ↦ Graph.sInter_le (hle hGs)
-
-def Equiv.insert_option {s : Set α} [DecidablePred fun (x : α) => x ∈ s] (a : α) (has : a ∉ s) :
-    Option s ≃ (insert a s : Set α) :=
-  (Equiv.optionEquivSumPUnit _).trans (Equiv.Set.insert has).symm
-
-protected lemma sInter_insert_eq_iInter {s : Set (Graph α β)} [DecidablePred (· ∈ s)]
-    (hGs : G ∉ s) : Graph.sInter (insert G s) (by simp) = Graph.iInter
-    ((fun G : (insert G s : Set _) ↦ G.1) ∘ (Equiv.insert_option G hGs)) :=
-  Graph.iInter_comp_eq_of_surj <| Equiv.surjective (Equiv.insert_option G hGs)
-
-protected lemma sInter_image {s : Set ι} (hne : s.Nonempty) (f : ι → Graph α β) :
-    Graph.sInter (f '' s) (by simpa) = @Graph.iInter _ _ _ hne.to_subtype (f · : s → _) := by
-  rw [Graph.sInter]
-  let f' : s → ↑(f '' s) := fun i ↦ ⟨f i, ⟨i, i.2, rfl⟩⟩
-  have := hne.to_subtype
-  exact Graph.iInter_comp_eq_of_surj (f := f') fun ⟨_, i, hGs, rfl⟩ ↦ ⟨⟨i, hGs⟩, rfl⟩
-
-protected lemma sInter_range [Nonempty ι] {f : ι → Graph α β} :
-    Graph.sInter (Set.range f) (range_nonempty f) = .iInter f := by
-  rw [Graph.sInter]
-  exact Graph.iInter_comp_eq_of_surj (f := Set.rangeFactorization f) surjective_onto_range
-
-@[simp]
-protected lemma sInter_singleton (G : Graph α β) : Graph.sInter {G} (by simp) = G := by
-  apply le_antisymm (Graph.sInter_le (by simp))
-  rw [Graph.le_sInter_iff (by simp)]
-  exact fun G_2 a ↦ Eq.ge a
-
-@[simp]
-lemma sInter_inc_iff {s : Set (Graph α β)} (hs : s.Nonempty) :
-    (Graph.sInter s hs).Inc e x ↔ ∃ y, ∀ G ∈ s, G.IsLink e x y := by
-  simp only [Inc, sInter_isLink]
-
-@[simp]
-lemma sInter_isLoopAt_iff {s : Set (Graph α β)} (hs : s.Nonempty) :
-    (Graph.sInter s hs).IsLoopAt e x ↔ ∀ G ∈ s, G.IsLoopAt e x := by
-  simp only [IsLoopAt, sInter_isLink]
-
-@[simp]
-lemma sInter_isNonloopAt_iff {s : Set (Graph α β)} (hs : s.Nonempty) :
-    (Graph.sInter s hs).IsNonloopAt e x ↔ ∃ y ≠ x, ∀ G ∈ s, G.IsLink e x y := by
-  simp only [IsNonloopAt, sInter_isLink]
-
-@[simp]
-lemma induce_sInter {s : Set (Graph α β)} (hs : s.Nonempty) (X : Set α) :
-    (Graph.sInter s hs)[X] = .sInter ((·[X]) '' s) (by simpa) := by
-  refine Graph.ext (by simp; exact (biInter_const hs X).symm) fun e x y ↦ ?_
-  simp +contextual only [induce_isLink_iff, sInter_isLink, mem_image, forall_exists_index, and_imp,
-    forall_apply_eq_imp_iff₂, iff_def, and_self, implies_true, true_and]
-  exact fun h ↦ (h _ hs.some_mem).right
-
-@[simp]
-lemma vertexDelete_sInter {s : Set (Graph α β)} (hs : s.Nonempty) (X : Set α) :
-    (Graph.sInter s hs) - X = .sInter ((· - X) '' s) (by simpa) := by
-  refine Graph.ext (by simp [biInter_diff_distrib hs]) fun e x y ↦ ?_
-  simp +contextual only [vertexDelete_isLink_iff, sInter_isLink, mem_image, forall_exists_index,
-    and_imp, forall_apply_eq_imp_iff₂, iff_def, not_false_eq_true, and_self, implies_true, true_and]
-  exact fun h ↦ (h _ hs.some_mem).right
-
-@[simp]
-lemma edgeDelete_sInter {s : Set (Graph α β)} (hs : s.Nonempty) (F : Set β) :
-    (Graph.sInter s hs) ＼ F = .sInter ((· ＼ F) '' s) (by simpa) :=
-  Graph.ext (by simp [biInter_diff_distrib hs]) fun e x y ↦ by
-  simp +contextual only [edgeDelete_isLink, sInter_isLink, mem_image, forall_exists_index, and_imp,
-    forall_apply_eq_imp_iff₂, iff_def, not_false_eq_true, and_self, implies_true, true_and]
-  exact fun h ↦ (h _ hs.some_mem).right
-
-@[simp]
-lemma edgeRestrict_sInter {s : Set (Graph α β)} (hs : s.Nonempty) (F : Set β) :
-    (Graph.sInter s hs) ↾ F = .sInter ((· ↾ F) '' s) (by simpa) :=
-  Graph.ext (by simp [biInter_diff_distrib hs]) fun e x y ↦ by
-  simp +contextual only [edgeRestrict_isLink, sInter_isLink, mem_image, forall_exists_index,
-    and_imp, forall_apply_eq_imp_iff₂, iff_def, and_self, implies_true, and_true, true_and]
-  exact fun h ↦ (h _ hs.some_mem).left
-
-/-! ### Intersections -/
-
-/-- The intersection of two graphs `G` and `H`. There seems to be no good way to
-defined junk values so that this has the right edge and vertex set, so the
-edges are precisely those on which `G` and `H` agree, and the edge set is a subset
-of `E(G) ∩ E(H)`,
-with equality if `G` and `H` are compatible.   -/
-protected def inter (G H : Graph α β) : Graph α β where
-  vertexSet := V(G) ∩ V(H)
-  IsLink e x y := G.IsLink e x y ∧ H.IsLink e x y
-  isLink_symm _ _ _ _ h := ⟨h.1.symm, h.2.symm⟩
-  dup_or_dup_of_isLink_of_isLink _ _ _ _ _ h h' := h.1.left_eq_or_eq h'.1
-  edge_mem_iff_exists_isLink e := by simp
-  left_mem_of_isLink e x y h := ⟨h.1.left_mem, h.2.left_mem⟩
-
-instance : Inter (Graph α β) where inter := Graph.inter
-
-@[simp]
-lemma inter_vertexSet (G H : Graph α β) : V(G ∩ H) = V(G) ∩ V(H) := rfl
-
-@[simp]
-lemma inter_isLink_iff : (G ∩ H).IsLink e x y ↔ G.IsLink e x y ∧ H.IsLink e x y := Iff.rfl
-
-protected lemma inter_comm (G H : Graph α β) : G ∩ H = H ∩ G :=
-  Graph.ext (Set.inter_comm ..) <| by simp [and_comm]
-
-lemma inter_edgeSet (G H : Graph α β) :
-    E(G ∩ H) = {e ∈ E(G) ∩ E(H) | G.IsLink e = H.IsLink e} := by
-  simp only [edgeSet_eq_setOf_exists_isLink, inter_isLink_iff, mem_inter_iff, mem_setOf_eq,
-    funext_iff, eq_iff_iff, Set.ext_iff]
-  exact fun e ↦ ⟨fun ⟨x, y, hfG, hfH⟩ ↦ ⟨⟨⟨_, _, hfG⟩, ⟨_, _, hfH⟩⟩,
-    fun z w ↦ by rw [hfG.isLink_iff_sym2_eq, hfH.isLink_iff_sym2_eq]⟩,
-    fun ⟨⟨⟨x, y, hexy⟩, ⟨z, w, hezw⟩⟩, h⟩ ↦ ⟨x, y, hexy, by rwa [← h]⟩⟩
-
-lemma inter_edgeSet_subset : E(G ∩ H) ⊆ E(G) ∩ E(H) := by
-  simp +contextual [inter_edgeSet, subset_def]
-
-@[simp]
-lemma inter_inc_iff : (G ∩ H).Inc e x ↔ ∃ y, G.IsLink e x y ∧ H.IsLink e x y := by
+lemma union_inc_iff : (G ∪ H).Inc e x ↔ ∃ u, (G.Inc e u ∨ (H.Inc e u ∧ e ∉ E(G))) ∧
+    Relation.TransGen (G.dup ⊔ H.dup) x u := by
   simp [Inc]
-
-@[simp]
-lemma inter_isLoopAt_iff : (G ∩ H).IsLoopAt e x ↔ G.IsLoopAt e x ∧ H.IsLoopAt e x := by
-  simp [← isLink_self_iff]
-
-@[simp]
-lemma inter_isNonloopAt_iff :
-    (G ∩ H).IsNonloopAt e x ↔ ∃ y ≠ x, G.IsLink e x y ∧ H.IsLink e x y := by
-  simp [IsNonloopAt]
-
-@[simp]
-protected lemma inter_le_left : G ∩ H ≤ G where
-  vertex_subset := inter_subset_left
-  isLink_of_isLink := by simp +contextual
-
-@[simp]
-protected lemma inter_le_right : G ∩ H ≤ H :=
-  Graph.inter_comm _ _ ▸ Graph.inter_le_left
-
-protected lemma le_inter (h₁ : H ≤ G₁) (h₂ : H ≤ G₂) : H ≤ G₁ ∩ G₂ where
-  vertex_subset := subset_inter (vertexSet_mono h₁) (vertexSet_mono h₂)
-  isLink_of_isLink e x y h := by simp [h.of_le h₁, h.of_le h₂]
-
-instance : SemilatticeInf (Graph α β) where
-  inf := Graph.inter
-  inf_le_left _ _ := Graph.inter_le_left
-  inf_le_right _ _ := Graph.inter_le_right
-  le_inf _ _ _ := Graph.le_inter
-
-@[simp]
-lemma inf_eq_inter : H₁ ⊓ H₂ = H₁ ∩ H₂ := rfl
-
-@[simp]
-lemma inter_eq_bot_iff : H₁ ∩ H₂ = ⊥ ↔ V(H₁) ∩ V(H₂) = ∅ := by
-  rw [← vertexSet_eq_empty_iff, inter_vertexSet]
-
-lemma disjoint_iff_inter_eq_bot : Disjoint H₁ H₂ ↔ H₁ ∩ H₂ = ⊥ := by
-  rw [disjoint_iff, inf_eq_inter]
-
-@[simp]
-lemma disjoint_iff_vertexSet_inter_eq_empty : Disjoint H₁ H₂ ↔ V(H₁) ∩ V(H₂) = ∅ := by
-  rw [disjoint_iff_inter_eq_bot, inter_eq_bot_iff]
-
-lemma disjoint_iff_vertexSet_disjoint : Disjoint H₁ H₂ ↔ Disjoint V(H₁) V(H₂) := by
-  rw [disjoint_iff_inter_eq_bot, inter_eq_bot_iff, Set.disjoint_iff_inter_eq_empty]
-
-alias ⟨Disjoint.vertex_disjoint, _⟩ := disjoint_iff_vertexSet_disjoint
-
-lemma Compatible.inter_edgeSet (h : G.Compatible H) : E(G ∩ H) = E(G) ∩ E(H) := by
-  rw [Graph.inter_edgeSet]
-  exact le_antisymm (fun e he ↦ he.1) fun e he ↦ ⟨he, h he⟩
-
-lemma inter_eq_iInter : G ∩ H = Graph.iInter (fun b ↦ bif b then G else H) :=
-  Graph.ext (by simp [Set.inter_eq_iInter, Bool.apply_cond]) (by simp [and_comm])
-
-lemma le_inter_iff : H ≤ G₁ ∩ G₂ ↔ H ≤ G₁ ∧ H ≤ G₂ := by
-  simp [inter_eq_iInter, and_comm]
-
-lemma inter_eq_self_of_le (hle : G ≤ H) : G ∩ H = G :=
-  le_antisymm Graph.inter_le_left <| by simpa [le_inter_iff]
-
-lemma le_of_inter_eq_self (h : G ∩ H = G) : G ≤ H := by
-  rw [← h]
-  exact Graph.inter_le_right
-
-lemma inter_mono_left (hle : G₁ ≤ G₂) : G₁ ∩ H ≤ G₂ ∩ H := by
-  rw [le_inter_iff]
-  exact ⟨Graph.inter_le_left.trans hle, Graph.inter_le_right⟩
-
-lemma inter_mono_right (hle : H₁ ≤ H₂) : G ∩ H₁ ≤ G ∩ H₂ := by
-  rw [le_inter_iff]
-  exact ⟨Graph.inter_le_left, Graph.inter_le_right.trans hle⟩
-
-lemma inter_mono (hleG : G₁ ≤ G₂) (hleH : H₁ ≤ H₂) : G₁ ∩ H₁ ≤ G₂ ∩ H₂ :=
-  (inter_mono_right hleH).trans (inter_mono_left hleG)
-
-lemma stronglyDisjoint_iff_disjoint_of_compatible (h : H₁.Compatible H₂) :
-    StronglyDisjoint H₁ H₂ ↔ Disjoint H₁ H₂ := by
-  rw [stronglyDisjoint_iff_vertexSet_disjoint_compatible, Set.disjoint_iff_inter_eq_empty,
-    disjoint_iff, ← vertexSet_eq_empty_iff]
-  simp [h]
-
-lemma edgeSet_induce_inter_eq_edgeSet_induce_of_le (h : G ≤ H) : E(G) ∩ E(H[X]) = E(G[X]) :=
-  Set.ext fun _ ↦ ⟨fun ⟨he, x, y, hl, hx, hy⟩ => ⟨x, y, hl.of_le_of_mem h he, hx, hy⟩,
-    fun ⟨x, y, hl, hx, hy⟩ => ⟨hl.edge_mem, x, y, hl.of_le h, hx, hy⟩⟩
-
-lemma induce_inter (X Y : Set α) : G[X ∩ Y] = G[X] ∩ G[Y] :=
-  Graph.ext (by simp) fun e x y ↦ by
-  simp +contextual only [induce_isLink_iff, mem_inter_iff, inter_isLink_iff, iff_def, and_self,
-    implies_true]
-
-lemma induce_inter_distrib (X : Set α) : (G ∩ H)[X] = G[X] ∩ H[X] :=
-  Graph.ext (by simp) fun e x y ↦ by
-  simp +contextual only [induce_isLink_iff, inter_isLink_iff, iff_def, and_self, implies_true]
-
-lemma vertexDelete_union (X Y : Set α) : G - (X ∪ Y) = (G - X) ∩ (G - Y) :=
-  Graph.ext (by simp [diff_inter_diff]) fun e x y ↦ by
-  simp +contextual only [vertexDelete_isLink_iff, mem_union, not_or, inter_isLink_iff, iff_def,
-    not_false_eq_true, and_self, implies_true]
-
-lemma vertexDelete_inter_distrib (X : Set α) : (G ∩ H) - X = (G - X) ∩ (H - X) :=
-  Graph.ext (by simp [diff_inter_distrib_right]) fun e x y ↦ by
-  simp +contextual only [vertexDelete_isLink_iff, inter_isLink_iff, iff_def, not_false_eq_true,
-    and_self, implies_true]
-
-lemma edgeDelete_union (F₁ F₂ : Set β) : G ＼ (F₁ ∪ F₂) = (G ＼ F₁) ∩ (G ＼ F₂) :=
-  Graph.ext (by simp [diff_inter_diff]) fun e x y ↦ by
-  simp +contextual only [edgeDelete_isLink, mem_union, not_or, inter_isLink_iff, iff_def,
-    not_false_eq_true, and_self, implies_true]
-
-lemma edgeDelete_inter_distrib (F : Set β) : (G ∩ H) ＼ F = (G ＼ F) ∩ (H ＼ F) :=
-  Graph.ext (by simp) fun e x y ↦ by
-  simp +contextual only [edgeDelete_isLink, inter_isLink_iff, iff_def, not_false_eq_true, and_self,
-    implies_true]
-
-lemma edgeRestrict_inter (F₁ F₂ : Set β) : (G ↾ (F₁ ∩ F₂)) = (G ↾ F₁) ∩ (G ↾ F₂) :=
-  Graph.ext (by simp) fun e x y ↦ by
-  simp +contextual only [edgeRestrict_isLink, mem_inter_iff, inter_isLink_iff, iff_def, and_self,
-    implies_true]
-
-lemma edgeRestrict_inter_distrib (F : Set β) : (G ∩ H) ↾ F = (G ↾ F) ∩ (H ↾ F) :=
-  Graph.ext (by simp) fun e x y ↦ by
-  simp +contextual only [edgeRestrict_isLink, inter_isLink_iff, iff_def, and_self, implies_true]
-
-protected lemma inter_distrib_iInter [Nonempty ι] {H : ι → Graph α β} :
-    G ∩ (Graph.iInter H) = Graph.iInter (fun i ↦ G ∩ (H i)) :=
-  Graph.ext (by simp [inter_iInter]) (by
-    simp only [inter_isLink_iff, iInter_isLink]
-    rintro i x y
-    rw [forall_and_left])
-
-protected lemma inter_distrib_sInter [Nonempty ι] {s : Set (Graph α β)} (hne : s.Nonempty) :
-    G ∩ (Graph.sInter s hne) = Graph.sInter ((G ∩ ·) '' s) (by simpa) := by
-  rw [Graph.sInter_image hne]
-  unfold Graph.sInter
-  have := hne.to_subtype
-  rw [Graph.inter_distrib_iInter]
-
-protected lemma inter_distrib_iUnion {H : ι → Graph α β} (hH : Pairwise (Compatible on H)) :
-    G ∩ (Graph.iUnion H hH) = Graph.iUnion (fun i ↦ G ∩ (H i))
-      (fun _ _ hne ↦ (hH hne).mono Graph.inter_le_right Graph.inter_le_right) :=
-  Graph.ext (by simp [inter_iUnion]) (by simp)
-
-protected lemma inter_distrib_sUnion (hs : s.Pairwise Compatible) :
-    G ∩ (Graph.sUnion s hs) = Graph.sUnion ((fun K ↦ G ∩ K) '' s) (by
-      rintro _ ⟨K₁, hK₁, rfl⟩ _ ⟨K₂, hK₂, rfl⟩ -
-      exact (hs.of_refl hK₁ hK₂).mono Graph.inter_le_right Graph.inter_le_right) := by
-  ext <;> aesop
-
-lemma Pairwise.union_compatible {s t : Set (Graph α β)} (hst : (s ∪ t).Pairwise Compatible) :
-    (Graph.sUnion s (hst.mono subset_union_left)).Compatible
-    (Graph.sUnion t (hst.mono subset_union_right)) := by
-  refine compatible_of_le_le (G := Graph.sUnion (s ∪ t) hst) ?_ ?_ <;> rw [Graph.sUnion_le_iff]
-  <;> exact fun G hG ↦ Graph.le_sUnion hst (by simp [hG])
-
-lemma sUnion_union_sUnion {s t : Set (Graph α β)} (hst : (s ∪ t).Pairwise Compatible) :
-    Graph.sUnion s (hst.mono subset_union_left) ∪ Graph.sUnion t (hst.mono subset_union_right) =
-    Graph.sUnion (s ∪ t) hst := by
-  have hs : s.Pairwise Compatible := hst.mono subset_union_left
-  have ht : t.Pairwise Compatible := hst.mono subset_union_right
-  refine Graph.ext (by aesop) fun e x y ↦ ?_
-  rw [(Pairwise.union_compatible hst).union_isLink_iff]
-  aesop
-
-protected lemma sInter_inter_sInter {s t : Set (Graph α β)} (hs : s.Nonempty) (ht : t.Nonempty) :
-    Graph.sInter s hs ∩ .sInter t ht = .sInter (s ∪ t) (by simp [hs]) := by
-  ext <;> aesop
-
-lemma Compatible.sum_compatible {G : ι → Graph α β} {H : ι' → Graph α β}
-    (hGH : Pairwise (Compatible on (Sum.elim G H))) :
-    (Graph.iUnion G (hGH.sum_left)).Compatible (Graph.iUnion H (hGH.sum_right)) :=
-  compatible_of_le_le (iUnion_left_le_iUnion_sum hGH) <| iUnion_right_le_iUnion_sum hGH
-
-protected lemma iUnion_sum [Nonempty ι] [Nonempty ι'] {G : ι → Graph α β}
-    {H : ι' → Graph α β} (hGH : Pairwise (Compatible on (Sum.elim G H))) :
-    Graph.iUnion (Sum.elim G H) hGH = (.iUnion G hGH.sum_left) ∪ (.iUnion H hGH.sum_right) := by
-  refine le_antisymm ?_ <| Graph.union_le (iUnion_left_le_iUnion_sum hGH)
-    (iUnion_right_le_iUnion_sum hGH)
-  rw [Graph.iUnion_le_iff]
-  rintro (i | i) <;> simp only [Sum.elim_inl, Sum.elim_inr]
-  · exact le_trans (Graph.le_iUnion hGH.sum_left i) (Graph.left_le_union _ _)
-  · exact le_trans (Graph.le_iUnion hGH.sum_right i)
-      (Compatible.right_le_union (Compatible.sum_compatible hGH))
-
-protected lemma iInter_sum [Nonempty ι] [Nonempty ι'] {G : ι → Graph α β}
-    {H : ι' → Graph α β} : Graph.iInter (Sum.elim G H) = .iInter G ∩ .iInter H := by
-  ext <;> aesop
-
-protected lemma iInter_option [Nonempty ι] {G₁ : Graph α β} {G : ι → Graph α β} :
-    Graph.iInter (Option.elim · G₁ G) = G₁ ∩ Graph.iInter G :=
-  Graph.ext (by simp [Set.iInter_option]) (by simp [Option.forall])
-
-protected lemma sInter_insert {s : Set (Graph α β)} (G : Graph α β) (hne : s.Nonempty) :
-    Graph.sInter (insert G s) (by simp) = G ∩ Graph.sInter s hne := by
-  ext v <;> simp
-
-lemma iInter_option_eq_sInter_insert {G₁ : Graph α β} {G : ι → Graph α β} :
-    Graph.iInter (Option.elim · G₁ G) = Graph.sInter (insert G₁ (range G)) (by simp) := by
-  obtain hι | hι := isEmpty_or_nonempty ι
-  · simp [range_eq_empty G]
-  rw [Graph.sInter_insert _ (range_nonempty _), Graph.sInter_range, Graph.iInter_option]
-
--- protected lemma union_iInter [Nonempty ι] {H : ι → Graph α β} (hc : ∀ i, G.Compatible (H i))
---     (hH : Pairwise (Compatible on H)) :
---     G ∪ (Graph.iInter H hH) = Graph.iInter (fun i ↦ G ∪ (H i))
---     (by
---       refine fun i j hij ↦ (h)
---     )
-
---     := by
---   _
-
-  -- rw [Graph.sUnion, Graph.sUnion]
-  -- generalize_proofs h₁ h₂
-  -- rw [Graph.inter_distrib_iUnion _]
-
-
-
-
-
-section Subgraph
-
-/-! ### Subgraphs -/
-
-variable {H : ι → Graph α β} {H₁ H₂ : Graph α β}
-
-lemma pairwise_compatible_of_subgraph {H : ι → Graph α β} (h : ∀ i, H i ≤ G) :
-    Pairwise (Compatible on H) :=
-  fun i j _ ↦ compatible_of_le_le (h i) (h j)
-
-lemma set_pairwise_compatible_of_subgraph (h : ∀ ⦃H⦄, H ∈ s → H ≤ G) :
-    s.Pairwise Compatible :=
-  fun _ hi _ hj _ ↦ compatible_of_le_le (h hi) (h hj)
-
-protected lemma iUnion_le_of_forall_le (h : ∀ i, H i ≤ G) :
-    Graph.iUnion H (pairwise_compatible_of_subgraph h) ≤ G := by
-  simpa
-
-protected lemma sUnion_le_of_forall_le (h : ∀ ⦃H⦄, H ∈ s → H ≤ G) :
-    Graph.sUnion s (set_pairwise_compatible_of_subgraph h) ≤ G := by
-  simpa
-
-protected lemma iInter_le_of_forall_le [Nonempty ι] (h : ∀ i, H i ≤ G) :
-    Graph.iInter H ≤ G :=
-  (Graph.iInter_le (Classical.arbitrary ι)).trans <| h _
-
-protected lemma sInter_le_of_forall_le (h : ∀ ⦃H⦄, H ∈ s → H ≤ G) (hne : s.Nonempty) :
-    Graph.sInter s hne ≤ G :=
-  have := hne.to_subtype
-  Graph.iInter_le_of_forall_le (by simpa)
-
-/-- A union of closed subgraphs of `G` is a closed subgraph of `G`. -/
-lemma iUnion_isClosedSubgraph (h : ∀ i, H i ≤c G) :
-    Graph.iUnion H (pairwise_compatible_of_subgraph (fun i ↦ (h i).le)) ≤c G where
-  le := Graph.iUnion_le_of_forall_le fun i ↦ (h i).le
-  closed e x he := by
-    simp only [iUnion_vertexSet, mem_iUnion, iUnion_edgeSet, forall_exists_index]
-    exact fun i hxi ↦ ⟨_, (he.of_isClosedSubgraph_of_mem (h i) hxi).edge_mem⟩
-
-/-- A nonempty union of spanning subgraphs of `G` is a spanning subgraph of `G`. -/
-lemma iUnion_isSpanningSubgraph [Nonempty ι] (h : ∀ i, H i ≤s G) :
-    Graph.iUnion H (pairwise_compatible_of_subgraph (fun i ↦ (h i).le)) ≤s G where
-  le := Graph.iUnion_le_of_forall_le fun i ↦ (h i).le
-  vertexSet_eq := by simp [(h _).vertexSet_eq, iUnion_const]
-
--- A weakening of the previous lemma.
-lemma iUnion_isSpanningSubgraph_of_exists_isSpanningSubgraph_of_forall_le [Nonempty ι]
-    (h : ∀ i, H i ≤ G) (hH : ∃ i, H i ≤s G) :
-    Graph.iUnion H (pairwise_compatible_of_subgraph h) ≤s G where
-  le := Graph.iUnion_le_of_forall_le h
-  vertexSet_eq := by
-    apply le_antisymm
-    · simp only [iUnion_vertexSet, le_eq_subset, iUnion_subset_iff]
-      exact fun i ↦ (h i).vertex_subset
-    obtain ⟨i, hi⟩ := hH
-    rw [← hi.vertexSet_eq]
-    exact subset_iUnion_of_subset i fun ⦃a⦄ a ↦ a
-
-/-- A nonempty intersection of induced subgraphs `G` is an induced subgraph of `G`-/
-lemma iInter_isInducedSubgraph [Nonempty ι] (h : ∀ i, H i ≤i G) :
-    Graph.iInter H ≤i G where
-  le := Graph.iInter_le_of_forall_le fun i ↦ (h i).le
-  isLink_of_mem_mem := by
-    simp only [iInter_vertexSet, mem_iInter, iInter_isLink]
-    exact fun e x y he hx hy i ↦ (h i).isLink_of_mem_mem he (hx i) (hy i)
-
-/-- A nonempty intersection of spanning subgraphs of `G` is a spanning subgraph of `G`.-/
-lemma iInter_isSpanningSubgraph [Nonempty ι] (h : ∀ i, H i ≤s G) :
-    Graph.iInter H ≤s G where
-  le := Graph.iInter_le_of_forall_le fun i ↦ (h i).le
-  vertexSet_eq := iInter_eq_const fun i ↦ (h i).vertexSet_eq
-
-/-- A nonempty intersection of closed subgraphs `G` is an induced subgraph of `G`-/
-lemma iInter_isClosedSubgraph [Nonempty ι] (h : ∀ i, H i ≤c G) :
-    Graph.iInter H ≤c G where
-  le := Graph.iInter_le_of_forall_le fun i ↦ (h i).le
-  closed e x he := by
-    simp only [iInter_vertexSet, mem_iInter, iInter_edgeSet, mem_setOf_eq]
-    rintro hx
-    obtain ⟨y, hy⟩ := he
-    use x, y, fun i ↦ by rwa [(h i).isLink_iff_of_mem (hx i)]
-
-lemma sUnion_isClosedSubgraph (hs : ∀ ⦃H⦄, H ∈ s → H ≤c G) :
-    Graph.sUnion s (set_pairwise_compatible_of_subgraph (fun _ h ↦ (hs h).le)) ≤c G :=
-  iUnion_isClosedSubgraph <| by simpa
-
-lemma sUnion_isSpanningSubgraph (hs : ∀ ⦃H⦄, H ∈ s → H ≤s G) (hne : s.Nonempty) :
-    Graph.sUnion s (set_pairwise_compatible_of_subgraph (fun _ h ↦ (hs h).le)) ≤s G :=
-  have := hne.to_subtype
-  iUnion_isSpanningSubgraph <| by simpa
-
-lemma sInter_isInducedSubgraph (hs : ∀ ⦃H⦄, H ∈ s → H ≤i G) (hne : s.Nonempty) :
-    Graph.sInter s hne ≤i G :=
-  have := hne.to_subtype
-  iInter_isInducedSubgraph <| by simpa
-
-lemma sInter_isClosedSubgraph (hs : ∀ ⦃H⦄, H ∈ s → H ≤c G) (hne : s.Nonempty) :
-    Graph.sInter s hne ≤c G :=
-  have := hne.to_subtype
-  iInter_isClosedSubgraph <| by simpa
-
-lemma isClosedSubgraph_iUnion_of_stronglyDisjoint (h : Pairwise (StronglyDisjoint on H)) (i : ι) :
-    H i ≤c Graph.iUnion H (h.mono fun _ _ ↦ StronglyDisjoint.compatible) where
-  le := Graph.le_iUnion ..
-  closed e x he hx := by
-    obtain ⟨j, hj : (H j).Inc e x⟩ := (iUnion_inc_iff ..).1 he
-    obtain rfl | hne := eq_or_ne i j
-    · exact hj.edge_mem
-    exact False.elim <| (h hne).vertex.notMem_of_mem_left hx hj.vertex_mem
-
-lemma isClosedSubgraph_sUnion_of_stronglyDisjoint (s : Set (Graph α β))
-    (hs : s.Pairwise StronglyDisjoint) (hG : G ∈ s) : G ≤c Graph.sUnion s (hs.mono' (by simp)) :=
-  isClosedSubgraph_iUnion_of_stronglyDisjoint ((pairwise_subtype_iff_pairwise_set ..).2 hs) ⟨G, hG⟩
-
-lemma isClosedSubgraph_union_left_of_vertexSet_disjoint (h : Disjoint V(H₁) V(H₂)) :
-    H₁ ≤c H₁ ∪ H₂ := by
-  refine ⟨Graph.left_le_union H₁ H₂, fun e x hinc hx₁ => ?_⟩
-  have hninc : ¬ H₂.Inc e x := fun hinc ↦ h.notMem_of_mem_left hx₁ hinc.vertex_mem
-  simp only [union_inc_iff, hninc, false_and, or_false] at hinc
-  exact hinc.edge_mem
-
-lemma Disjoint.isClosedSubgraph_union_left (h : Disjoint H₁ H₂) : H₁ ≤c H₁ ∪ H₂ :=
-  isClosedSubgraph_union_left_of_vertexSet_disjoint <| Disjoint.vertex_disjoint h
-
-lemma StronglyDisjoint.isClosedSubgraph_union_left (h : StronglyDisjoint H₁ H₂) :
-    H₁ ≤c H₁ ∪ H₂ := by
-  rw [(stronglyDisjoint_le_compatible _ _ h).union_eq_sUnion]
-  exact isClosedSubgraph_sUnion_of_stronglyDisjoint _ (by simp [Set.Pairwise, h, h.symm]) (by simp)
-
-lemma StronglyDisjoint.isClosedSubgraph_union_right (h : StronglyDisjoint H₁ H₂) :
-    H₂ ≤c H₁ ∪ H₂ := by
-  rw [(stronglyDisjoint_le_compatible _ _ h).union_eq_sUnion]
-  exact isClosedSubgraph_sUnion_of_stronglyDisjoint _ (by simp [Set.Pairwise, h, h.symm]) (by simp)
-
-lemma IsClosedSubgraph.union (h₁ : H₁ ≤c G) (h₂ : H₂ ≤c G) : H₁ ∪ H₂ ≤c G := by
-  rw [(compatible_of_le_le h₁.le h₂.le).union_eq_iUnion]
-  exact iUnion_isClosedSubgraph <| by simp [h₁,h₂]
-
-lemma IsSpanningSubgraph.union (h₁ : H₁ ≤s G) (h₂ : H₂ ≤s G) : H₁ ∪ H₂ ≤s G := by
-  rw [(compatible_of_le_le h₁.le h₂.le).union_eq_iUnion]
-  exact iUnion_isSpanningSubgraph <| by simp [h₁,h₂]
-
-lemma IsSpanningSubgraph.union_left (h₁ : H₁ ≤s G) (h₂ : H₂ ≤ G) : H₁ ∪ H₂ ≤s G := by
-  rw [(compatible_of_le_le h₁.le h₂).union_eq_iUnion]
-  exact iUnion_isSpanningSubgraph_of_exists_isSpanningSubgraph_of_forall_le (by simp [h₁.le, h₂])
-    ⟨True, h₁⟩
-
-lemma IsSpanningSubgraph.union_right (h₁ : H₁ ≤ G) (h₂ : H₂ ≤s G) : H₁ ∪ H₂ ≤s G := by
-  rw [(compatible_of_le_le h₁ h₂.le).union_eq_iUnion]
-  exact iUnion_isSpanningSubgraph_of_exists_isSpanningSubgraph_of_forall_le (by simp [h₁, h₂.le])
-    ⟨False, h₂⟩
-
-lemma IsInducedSubgraph.inter (h₁ : H₁ ≤i G) (h₂ : H₂ ≤i G) : H₁ ∩ H₂ ≤i G := by
-  rw [inter_eq_iInter]
-  exact iInter_isInducedSubgraph <| by simp [h₁,h₂]
-
-lemma IsClosedSubgraph.inter (h₁ : H₁ ≤c G) (h₂ : H₂ ≤c G) : H₁ ∩ H₂ ≤c G := by
-  rw [inter_eq_iInter]
-  exact iInter_isClosedSubgraph <| by simp [h₁,h₂]
-
-lemma IsClosedSubgraph.inter_le {K G H : Graph α β} (hKG : K ≤c G) (hle : H ≤ G) : K ∩ H ≤c H where
-  le := Graph.inter_le_right
-  closed e x hex hx := by
-    rw [inter_vertexSet] at hx
-    have heK := ((hex.of_le hle).of_isClosedSubgraph_of_mem hKG hx.1).edge_mem
-    rw [(compatible_of_le_le hKG.le hle).inter_edgeSet]
-    exact ⟨heK, hex.edge_mem⟩
-
-@[simp]
-lemma le_bot_iff : G ≤ ⊥ ↔ G = ⊥ := _root_.le_bot_iff
-
-@[simp]
-lemma isClosedSubgraph_bot_iff : G ≤c ⊥ ↔ G = ⊥ :=
-  ⟨fun h => le_bot_iff.mp h.le, fun h => h ▸ bot_isClosedSubgraph ⊥⟩
-
-@[simp]
-lemma isSpanningSubgraph_bot_iff : G ≤s ⊥ ↔ G = ⊥ :=
-  ⟨fun h => le_bot_iff.mp h.le, fun h => h ▸ ⟨le_rfl, rfl⟩⟩
-
-@[simp]
-lemma isInducedSubgraph_bot_iff : G ≤i ⊥ ↔ G = ⊥ :=
-  ⟨fun h => le_bot_iff.mp h.le, fun h => h ▸ bot_isInducedSubgraph ⊥⟩
-
-@[simp]
-lemma induce_empty : G[∅] = ⊥ := by
-  rw [← vertexSet_eq_empty_iff, induce_vertexSet]
-
-end Subgraph
-
-/-! ### Adding one edge -/
-
-@[simp]
-lemma singleEdge_compatible_iff :
-    Compatible (Graph.singleEdge u v e) G ↔ (e ∈ E(G) → G.IsLink e u v) := by
-  refine ⟨fun h he ↦ by simp [← h ⟨by simp, he⟩], fun h f ⟨hfe, hf⟩ ↦ ?_⟩
-  obtain rfl : f = e := by simpa using hfe
-  ext x y
-  simp only [singleEdge_isLink, (h hf).isLink_iff]
-  tauto
-
-/-- Add a new edge `e` between vertices `a` and `b`. If `e` is already in the graph,
-its ends change to `a` and `b`. -/
-@[simps! edgeSet vertexSet]
-protected def addEdge (G : Graph α β) (e : β) (a b : α) : Graph α β :=
-  Graph.singleEdge a b e ∪ G
-
-lemma addEdge_isLink (G : Graph α β) (e : β) (a b : α) : (G.addEdge e a b).IsLink e a b := by
-  simp [Graph.addEdge, union_isLink_iff]
-
-lemma addEdge_isLink_of_ne (hf : G.IsLink f x y) (hne : f ≠ e) (a b : α) :
-    (G.addEdge e a b).IsLink f x y := by
-  simpa [Graph.addEdge, union_isLink_iff, hne]
-
-lemma addEdge_isLink_iff {a b : α} (he : e ∉ E(G)) :
-    (G.addEdge e a b).IsLink f x y ↔ (f = e ∧ s(a,b) = s(x,y)) ∨ G.IsLink f x y := by
-  have hc : Compatible (Graph.singleEdge x y e) G := by simp [he]
-  simp only [Graph.addEdge, union_isLink_iff, singleEdge_isLink, singleEdge_edgeSet,
-    mem_singleton_iff, edgeDelete_isLink, Sym2.eq, Sym2.rel_iff', Prod.mk.injEq, Prod.swap_prod_mk]
-  obtain rfl | hne := eq_or_ne e f
-  · have hl : ¬ G.IsLink e x y := fun h ↦ he h.edge_mem
-    simp only [true_and, not_true_eq_false, hl, and_self, or_false]
-    tauto
-  simp [hne.symm]
-
-lemma addEdge_deleteEdge (he : e ∉ E(G)) (hx : x ∈ V(G)) (hy : y ∈ V(G)) :
-    (G.addEdge e x y) ＼ {e} = G := by
-  have hc : Compatible (Graph.singleEdge x y e) G := by simp [he]
-  simp only [Graph.addEdge, Graph.ext_iff, edgeDelete_vertexSet, union_vertexSet,
-    singleEdge_vertexSet, union_eq_right, insert_subset_iff, hx, singleton_subset_iff, hy, and_self,
-    edgeDelete_isLink, hc.union_isLink_iff, singleEdge_isLink, mem_singleton_iff, true_and]
-  intro f p q
-  obtain rfl | hne := eq_or_ne f e
-  · suffices ¬ G.IsLink f p q by simpa
-    exact fun hf ↦ he hf.edge_mem
-  simp [hne]
-
-lemma addEdge_le (hle : H ≤ G) (he : G.IsLink e x y) : H.addEdge e x y ≤ G :=
-  Graph.union_le (by simpa) hle
-
-lemma le_addEdge (he : e ∉ E(G)) : G ≤ G.addEdge e x y :=
-  Compatible.right_le_union <| by simp [he]
-
-lemma addEdge_mono (hle : H ≤ G) : H.addEdge e x y ≤ G.addEdge e x y :=
-  union_mono_right hle
-
-lemma deleteEdge_le_addEdge : G ＼ {e} ≤ G.addEdge e x y := by
-  rw [Graph.addEdge, union_eq_union_edgeDelete]
-  simp only [singleEdge_edgeSet]
-  exact Compatible.right_le_union <| by simp
-
-lemma deleteEdge_addEdge : (G ＼ {e}).addEdge e x y = G.addEdge e x y := by
-  refine le_antisymm (addEdge_mono edgeDelete_le) ?_
-  unfold Graph.addEdge
-  rw [union_le_iff]
-  refine ⟨Graph.left_le_union (Graph.singleEdge x y e) (G ＼ {e}), Compatible.right_le_union ?_⟩
-  simp
-
-lemma addEdge_eq_self (hbtw : G.IsLink e x y) : G.addEdge e x y = G :=
-  le_antisymm (addEdge_le (by simp) hbtw) <| Compatible.right_le_union <| by simp [hbtw]
-
-lemma addEdge_idem : (G.addEdge e x y).addEdge e x y = G.addEdge e x y :=
-  addEdge_eq_self <| addEdge_isLink G e x y
-
-lemma isSpanningSubgraph_addEdge (he : e ∉ E(G)) (hx : x ∈ V(G)) (hy : y ∈ V(G)) :
-    G ≤s G.addEdge e x y := by
-  nth_rw 1 [← addEdge_deleteEdge he hx hy]
-  exact edgeDelete_isSpanningSubgraph
-
-lemma IsLink.deleteEdge_addEdge (h : G.IsLink e x y) : (G ＼ {e}).addEdge e x y = G :=
-  ext_of_le_le (addEdge_le (by simp) h) le_rfl (by simp [pair_subset_iff, h.left_mem, h.right_mem])
-    <| by simp [h.edge_mem]
+  refine ⟨fun ⟨y, u, v, h, hxu, hyv⟩ => ⟨u, h.imp (⟨v, ·⟩) fun ⟨h, he⟩ => ⟨⟨v, h⟩, he⟩, hxu⟩, ?_⟩
+  rintro ⟨u, (⟨v, h⟩ | ⟨⟨v, h⟩, he⟩), hxu⟩
+  · use v, u, v, Or.inl h, hxu
+    rw [← union_dup_refl_iff]
+    exact Or.inl h.right_mem
+  · use v, u, v, Or.inr ⟨h, he⟩, hxu
+    rw [← union_dup_refl_iff]
+    exact Or.inr h.right_mem
+
+-- lemma union_isLoopAt_iff : (G ∪ H).IsLoopAt e x ↔ G.IsLoopAt e x ∨ (H.IsLoopAt e x ∧ e ∉ E(G)) := by
+--   simp [union_eq_sUnion]
+
+-- lemma union_isNonloopAt_iff :
+--     (G ∪ H).IsNonloopAt e x ↔ G.IsNonloopAt e x ∨ (H.IsNonloopAt e x ∧ e ∉ E(G)) := by
+--   simp only [IsNonloopAt, ne_eq, union_isLink_iff]
+--   aesop
+
+-- lemma union_eq_union_edgeDelete (G H : Graph α β) : G ∪ H = G ∪ (H ＼ E(G)) := by
+--   simp [union_eq_sUnion, union_eq_sUnion]
+
+-- @[simp]
+-- protected lemma left_le_union (G H : Graph α β) : G ≤ G ∪ H := by
+--   simp_rw [le_iff, union_isLink_iff]
+--   tauto
+
+-- protected lemma union_le {H₁ H₂ : Graph α β} (h₁ : H₁ ≤ G) (h₂ : H₂ ≤ G) : H₁ ∪ H₂ ≤ G := by
+--   simp [union_eq_sUnion, h₁, edgeDelete_le.trans h₂]
+
+-- lemma union_le_iff {H₁ H₂ : Graph α β} : H₁ ∪ H₂ ≤ G ↔ H₁ ≤ G ∧ H₂ ＼ E(H₁) ≤ G := by
+--   simp [union_eq_sUnion]
+
+-- lemma union_mono_right (h : H₁ ≤ H₂) : G ∪ H₁ ≤ G ∪ H₂ := by
+--   simp only [union_eq_sUnion, Graph.sUnion_le_iff, mem_insert_iff, mem_singleton_iff,
+--     forall_eq_or_imp, forall_eq]
+--   exact ⟨Graph.le_sUnion _ (by simp), le_trans (edgeDelete_mono_left h) <|
+--     Graph.le_sUnion _ (by simp : H₂ ＼ E(G) ∈ _)⟩
+
+-- @[simp]
+-- protected lemma union_self (G : Graph α β) : G ∪ G = G :=
+--   (Graph.union_le le_rfl le_rfl).antisymm <| Graph.left_le_union ..
+
+-- protected lemma union_assoc (G₁ G₂ G₃ : Graph α β) : (G₁ ∪ G₂) ∪ G₃ = G₁ ∪ (G₂ ∪ G₃) := by
+--   refine Graph.ext (Set.union_assoc ..) fun e x y ↦ ?_
+--   simp [union_isLink_iff]
+--   tauto
+
+-- lemma isLink_or_isLink_of_union (h : (G ∪ H).IsLink e x y) : G.IsLink e x y ∨ H.IsLink e x y :=
+--   (union_isLink_iff.1 h).elim .inl fun h' ↦ .inr h'.1
+
+-- lemma Compatible.union_isLink_iff (h : G.Compatible H) :
+--     (G ∪ H).IsLink e x y ↔ G.IsLink e x y ∨ H.IsLink e x y := by
+--   by_cases heG : e ∈ E(G)
+--   · simp only [Graph.union_isLink_iff, heG, not_true_eq_false, and_false, or_false, iff_self_or]
+--     exact fun he ↦ by rwa [h.isLink_eq heG he.edge_mem]
+--   simp [heG, Graph.union_isLink_iff]
+
+-- lemma edgeRestrict_union (G : Graph α β) (F₁ F₂ : Set β) : (G ↾ (F₁ ∪ F₂)) = G ↾ F₁ ∪ (G ↾ F₂) := by
+--   refine Graph.ext (by simp) fun e x y ↦ ?_
+--   rw [(G.compatible_self.mono (by simp) (by simp)).union_isLink_iff]
+--   simp only [edgeRestrict_isLink, mem_union]
+--   tauto
+
+-- lemma Compatible.union_eq_sUnion (h : G.Compatible H) :
+--     G ∪ H = Graph.sUnion {G, H} (by simp [Set.pairwise_iff_of_refl, h, h.symm]) :=
+--   Graph.ext (by simp) fun e x y ↦ by simp [h.union_isLink_iff]
+
+-- lemma Compatible.union_inc_iff (h : G.Compatible H) : (G ∪ H).Inc e x ↔ G.Inc e x ∨ H.Inc e x := by
+--   simp_rw [Inc, h.union_isLink_iff]
+--   aesop
+
+-- lemma Compatible.union_isLoopAt_iff (h : G.Compatible H) :
+--     (G ∪ H).IsLoopAt e x ↔ G.IsLoopAt e x ∨ H.IsLoopAt e x := by
+--   simp_rw [← isLink_self_iff, h.union_isLink_iff]
+
+-- lemma Compatible.union_isNonloopAt_iff (h : G.Compatible H) :
+--     (G ∪ H).IsNonloopAt e x ↔ G.IsNonloopAt e x ∨ H.IsNonloopAt e x := by
+--   simp_rw [IsNonloopAt, h.union_isLink_iff]
+--   aesop
+
+-- lemma Compatible.union_adj_iff (h : G.Compatible H) : (G ∪ H).Adj x y ↔ G.Adj x y ∨ H.Adj x y := by
+--   simp [Adj, h.union_isLink_iff, exists_or]
+
+-- lemma Compatible.union_comm (h : Compatible G H) : G ∪ H = H ∪ G :=
+--   Graph.ext (Set.union_comm ..)
+--     fun _ _ _ ↦ by rw [h.union_isLink_iff, h.symm.union_isLink_iff, or_comm]
+
+-- lemma Compatible.union_le_iff {H₁ H₂ : Graph α β} (h_compat : H₁.Compatible H₂) :
+--     H₁ ∪ H₂ ≤ G ↔ H₁ ≤ G ∧ H₂ ≤ G := by
+--   simp [h_compat.union_eq_sUnion]
+
+-- lemma Compatible.right_le_union (h : G.Compatible H) : H ≤ G ∪ H := by
+--   simp [h.union_comm]
+
+-- lemma union_eq_self_of_le_left (hle : G ≤ H) : G ∪ H = H :=
+--   (Graph.union_le hle rfl.le).antisymm (H.compatible_self.mono_left hle).right_le_union
+
+-- lemma union_eq_self_of_le_right (hle : G ≤ H) : H ∪ G = H :=
+--   (Graph.union_le rfl.le hle).antisymm <| Graph.left_le_union ..
+
+-- lemma Compatible.union_mono_left (h : H₂.Compatible G) (hle : H₁ ≤ H₂) : H₁ ∪ G ≤ H₂ ∪ G := by
+--   rw [h.union_comm, (h.mono_left hle).union_comm]
+--   exact union_mono_right hle
+
+-- lemma Compatible.union_mono (hleG : G₁ ≤ G₂) (hleH : H₁ ≤ H₂) (h : G₂.Compatible H₁) :
+--     G₁ ∪ H₁ ≤ G₂ ∪ H₂ := le_trans (h.union_mono_left hleG) (union_mono_right hleH)
+
+-- lemma edgeRestrict_union_edgeDelete (G : Graph α β) (F : Set β) : (G ↾ F) ∪ (G ＼ F) = G := by
+--   rw [edgeDelete_eq_edgeRestrict, ← edgeRestrict_union, ← edgeRestrict_inter_edgeSet]
+--   simp only [union_diff_self, edgeRestrict_inter_edgeSet, edgeRestrict_union, edgeRestrict_self]
+--   exact union_eq_self_of_le_left (by simp)
+
+-- lemma edgeDelete_union_edgeRestrict (G : Graph α β) (F : Set β) : (G ＼ F) ∪ (G ↾ F) = G := by
+--   convert G.edgeRestrict_union_edgeDelete F using 1
+--   rw [Compatible.union_comm]
+--   apply G.compatible_of_le_le (by simp) (by simp)
+
+-- lemma induce_union_edgeDelete (G : Graph α β) (hX : X ⊆ V(G)) : G[X] ∪ (G ＼ E(G[X])) = G := by
+--   rw [← union_eq_union_edgeDelete, union_eq_self_of_le_left (induce_le hX)]
+
+-- lemma edgeDelete_union_induce (G : Graph α β) (hX : X ⊆ V(G)) : (G ＼ E(G[X])) ∪ G[X] = G := by
+--   rw [(Compatible.of_disjoint_edgeSet _).union_comm, induce_union_edgeDelete _ hX]
+--   simp [disjoint_sdiff_left]
+
+-- lemma Compatible.union_eq_iUnion (h : G.Compatible H) :
+--     G ∪ H = Graph.iUnion (fun b ↦ bif b then G else H) (by simpa [pairwise_on_bool]) := by
+--   generalize_proofs h'
+--   simp only [le_antisymm_iff, h.union_le_iff, Graph.iUnion_le_iff, Bool.forall_bool, cond_false,
+--     h.right_le_union, cond_true, Graph.left_le_union, and_self, and_true]
+--   exact ⟨Graph.le_iUnion h' true, Graph.le_iUnion h' false⟩
+
+-- lemma Compatible.induce_union (h : G.Compatible H) (X : Set α) : (G ∪ H)[X] = G[X] ∪ H[X] := by
+--   refine Graph.ext (by simp) fun e x y ↦ ?_
+--   simp only [induce_isLink_iff, h.union_isLink_iff, h.induce.union_isLink_iff]
+--   tauto
+
+-- lemma Compatible.vertexDelete_union (h : G.Compatible H) (X : Set α) :
+--     (G ∪ H) - X = (G - X) ∪ (H - X) := by
+--   simp only [h.union_eq_iUnion, vertexDelete_iUnion, Bool.apply_cond (f := fun G ↦ G - X),
+--     ← h.vertexDelete.union_eq_iUnion]
+
+-- lemma induce_union (G : Graph α β) (X Y : Set α) (hX : ∀ x ∈ X, ∀ y ∈ Y, ¬ G.Adj x y) :
+--     G [X ∪ Y] = G [X] ∪ G [Y] := by
+--   refine Graph.ext rfl fun e x y ↦ ?_
+--   simp only [induce_isLink_iff, mem_union, Compatible.induce_induce.union_isLink_iff]
+--   by_cases hxy : G.IsLink e x y
+--   · by_cases hx : x ∈ X
+--     · simp [hx, show y ∉ Y from fun hy ↦ hX x hx y hy hxy.adj]
+--     by_cases hy : y ∈ X
+--     · simp [hy, show x ∉ Y from fun hx ↦ hX _ hy _ hx hxy.symm.adj, hxy]
+--     simp [hx, hy]
+--   simp [hxy]
+
+-- /-! ### Indexed Intersections -/
+
+-- /-- The intersection of a nonempty family of pairwise compatible graphs.
+--   Remove any disagreeing edges. -/
+-- @[simps]
+-- protected def iInter [Nonempty ι] (G : ι → Graph α β) : Graph α β where
+--   vertexSet := ⋂ i, V(G i)
+--   dup x y := ∀ i, (G i).dup x y
+--   dup_refl_iff x := by simp [dup_refl_iff]
+--   dup_symm := by
+--     simp_rw [dup_comm]
+--     exact fun _ _ a ↦ a
+--   dup_trans x y z hxy hyz i := (hxy i).trans (hyz i)
+--   edgeSet := {e | ∃ x y, ∀ i, (G i).IsLink e x y}
+--   IsLink e x y := ∀ i, (G i).IsLink e x y
+--   isLink_symm e he x y := by simp [isLink_comm]
+--   dup_or_dup_of_isLink_of_isLink e u v x y h h' := by
+--     let i' := Classical.arbitrary ι
+--     obtain hux | huy := dup_or_dup_of_isLink_of_isLink _ (h i') (h' i')
+--     · sorry
+--     sorry
+--   edge_mem_iff_exists_isLink e := by simp
+--   left_mem_of_isLink e x y h := mem_iInter.2 fun i ↦ (h i).left_mem
+--   isLink_of_dup e x y z hxy hxz i := (hxy i |>.symm.isLink_left).mpr <| hxz i
+
+-- protected lemma iInter_le {G : ι → Graph α β} [Nonempty ι] (i : ι) : Graph.iInter G ≤ G i where
+--   vertex_subset := iInter_subset (fun i ↦ V(G i)) i
+--   isLink_of_isLink _ _ _ h := h i
+
+-- @[simp]
+-- lemma le_iInter_iff [Nonempty ι] {G : ι → Graph α β} :
+--     H ≤ Graph.iInter G ↔ ∀ i, H ≤ G i := by
+--   let j := Classical.arbitrary ι
+--   refine ⟨fun h i ↦ h.trans <| Graph.iInter_le .., fun h ↦ ?_⟩
+--   apply le_of_le_le_subset_subset (h j) (Graph.iInter_le ..) ?_ fun e he ↦ ?_
+--   · simp [fun i ↦ vertexSet_mono (h i)]
+--   simp only [iInter_edgeSet, mem_setOf_eq]
+--   obtain ⟨x, y, hbtw⟩ := exists_isLink_of_mem_edgeSet he
+--   use x, y, fun i ↦ hbtw.of_le (h i)
+
+-- @[simp]
+-- protected lemma iInter_const [Nonempty ι] (G : Graph α β) :
+--     Graph.iInter (fun (_ : ι) ↦ G) = G := by
+--   apply le_antisymm (Graph.iInter_le (Classical.arbitrary ι))
+--   rw [le_iInter_iff]
+--   exact fun i ↦ le_refl G
+
+-- lemma iInter_le_iUnion [Nonempty ι] {G : ι → Graph α β} (hG : Pairwise (Compatible on G)) :
+--     Graph.iInter G ≤ Graph.iUnion G hG :=
+--   (Graph.iInter_le (Classical.arbitrary ι)).trans <| Graph.le_iUnion ..
+
+-- protected lemma iInter_comp_le [Nonempty ι] [Nonempty ι'] {f : ι' → ι}
+--     {G : ι → Graph α β} : Graph.iInter G ≤ Graph.iInter (fun i ↦ G (f i)) := by
+--   rw [Graph.le_iInter_iff]
+--   exact fun i ↦ Graph.iInter_le (f i)
+
+-- lemma iInter_comp_eq_of_surj [Nonempty ι] [Nonempty ι'] {f : ι' → ι}
+--     {G : ι → Graph α β} (hf : Function.Surjective f) :
+--     Graph.iInter G = Graph.iInter (fun i ↦ G (f i)) :=
+--   le_antisymm (Graph.iInter_comp_le) <| by
+--   rw [Graph.le_iInter_iff]
+--   rintro i
+--   obtain ⟨i', rfl⟩ := hf i
+--   exact Graph.iInter_le i'
+
+-- lemma iInter_range [Nonempty ι'] {f : ι' → ι} {G : (Set.range f) → Graph α β} :
+--     Graph.iInter G = Graph.iInter (fun i ↦ G (Set.rangeFactorization f i)) :=
+--   iInter_comp_eq_of_surj surjective_onto_range
+
+-- @[simp]
+-- lemma iInter_inc_iff [Nonempty ι] {G : ι → Graph α β} :
+--     (Graph.iInter G).Inc e x ↔ ∃ y, ∀ i, (G i).IsLink e x y := by
+--   simp only [Inc, iInter_isLink]
+
+-- @[simp]
+-- lemma iInter_isLoopAt_iff [Nonempty ι] {G : ι → Graph α β} :
+--     (Graph.iInter G).IsLoopAt e x ↔ ∀ i, (G i).IsLoopAt e x := by
+--   simp only [IsLoopAt, iInter_isLink]
+
+-- @[simp]
+-- lemma iInter_isNonloopAt_iff [Nonempty ι] {G : ι → Graph α β} :
+--     (Graph.iInter G).IsNonloopAt e x ↔ ∃ y ≠ x, ∀ i, (G i).IsLink e x y := by
+--   simp only [IsNonloopAt, iInter_isLink]
+
+-- @[simp]
+-- lemma induce_iInter [Nonempty ι] {G : ι → Graph α β} (X : Set α) :
+--     (Graph.iInter G)[X] = .iInter (fun i ↦ (G i)[X]) :=
+--   Graph.ext (iInter_const X).symm fun e x y ↦ by
+--   simp [forall_and_right]
+
+-- @[simp]
+-- lemma vertexDelete_iInter [Nonempty ι] {G : ι → Graph α β} (X : Set α) :
+--     (Graph.iInter G) - X = .iInter (fun i ↦ (G i) - X) :=
+--   Graph.ext (by simp) fun e x y ↦ by
+--   simp +contextual only [vertexDelete_isLink_iff, iInter_isLink, iff_def, not_false_eq_true,
+--     and_self, implies_true, true_and]
+--   exact fun h ↦ (h <| Classical.arbitrary ι).right
+
+-- @[simp]
+-- lemma edgeDelete_iInter [Nonempty ι] {G : ι → Graph α β} (F : Set β) :
+--     (Graph.iInter G) ＼ F = .iInter (fun i ↦ (G i) ＼ F) :=
+--   Graph.ext (by simp) fun e x y ↦ by
+--   simp +contextual only [edgeDelete_isLink, iInter_isLink, iff_def, not_false_eq_true, and_self,
+--     implies_true, true_and]
+--   exact fun h ↦ (h <| Classical.arbitrary ι).right
+
+-- @[simp]
+-- lemma edgeRestrict_iInter [Nonempty ι] {G : ι → Graph α β} (F : Set β) :
+--     (Graph.iInter G) ↾ F = .iInter (fun i ↦ (G i) ↾ F) :=
+--   Graph.ext (by simp) fun e x y ↦ by
+--   simp +contextual only [edgeRestrict_isLink, iInter_isLink, iff_def, and_self, implies_true,
+--     and_true, true_and]
+--   exact fun h ↦ (h <| Classical.arbitrary ι).left
+
+-- /-! ### Set Intersections -/
+
+-- /-- The intersection of a nonempty set of pairwise compatible graphs. -/
+-- @[simps!]
+-- protected def sInter (s : Set (Graph α β)) (hne : s.Nonempty) :
+--     Graph α β :=
+--   @Graph.iInter _ _ _ hne.to_subtype (fun G : s ↦ G.1)
+
+-- protected lemma sInter_le {s : Set (Graph α β)} (hG : G ∈ s) :
+--     Graph.sInter s ⟨G, hG⟩ ≤ G := by
+--   rw [Graph.sInter]
+--   generalize_proofs h
+--   exact Graph.iInter_le (⟨G, hG⟩ : s)
+
+-- @[simp]
+-- protected lemma le_sInter_iff {s} (hne : s.Nonempty) :
+--     H ≤ Graph.sInter s hne ↔ ∀ G ∈ s, H ≤ G := by
+--   simp [Graph.sInter]
+
+-- protected lemma sInter_anti {s t : Set (Graph α β)} (hne : s.Nonempty) (hne' : t.Nonempty)
+--     (hle : s ⊆ t) : Graph.sInter t hne' ≤ Graph.sInter s hne := by
+--   rw [Graph.le_sInter_iff hne]
+--   exact fun G hGs ↦ Graph.sInter_le (hle hGs)
+
+-- def Equiv.insert_option {s : Set α} [DecidablePred fun (x : α) => x ∈ s] (a : α) (has : a ∉ s) :
+--     Option s ≃ (insert a s : Set α) :=
+--   (Equiv.optionEquivSumPUnit _).trans (Equiv.Set.insert has).symm
+
+-- protected lemma sInter_insert_eq_iInter {s : Set (Graph α β)} [DecidablePred (· ∈ s)]
+--     (hGs : G ∉ s) : Graph.sInter (insert G s) (by simp) = Graph.iInter
+--     ((fun G : (insert G s : Set _) ↦ G.1) ∘ (Equiv.insert_option G hGs)) :=
+--   Graph.iInter_comp_eq_of_surj <| Equiv.surjective (Equiv.insert_option G hGs)
+
+-- protected lemma sInter_image {s : Set ι} (hne : s.Nonempty) (f : ι → Graph α β) :
+--     Graph.sInter (f '' s) (by simpa) = @Graph.iInter _ _ _ hne.to_subtype (f · : s → _) := by
+--   rw [Graph.sInter]
+--   let f' : s → ↑(f '' s) := fun i ↦ ⟨f i, ⟨i, i.2, rfl⟩⟩
+--   have := hne.to_subtype
+--   exact Graph.iInter_comp_eq_of_surj (f := f') fun ⟨_, i, hGs, rfl⟩ ↦ ⟨⟨i, hGs⟩, rfl⟩
+
+-- protected lemma sInter_range [Nonempty ι] {f : ι → Graph α β} :
+--     Graph.sInter (Set.range f) (range_nonempty f) = .iInter f := by
+--   rw [Graph.sInter]
+--   exact Graph.iInter_comp_eq_of_surj (f := Set.rangeFactorization f) surjective_onto_range
+
+-- @[simp]
+-- protected lemma sInter_singleton (G : Graph α β) : Graph.sInter {G} (by simp) = G := by
+--   apply le_antisymm (Graph.sInter_le (by simp))
+--   rw [Graph.le_sInter_iff (by simp)]
+--   exact fun G_2 a ↦ Eq.ge a
+
+-- @[simp]
+-- lemma sInter_inc_iff {s : Set (Graph α β)} (hs : s.Nonempty) :
+--     (Graph.sInter s hs).Inc e x ↔ ∃ y, ∀ G ∈ s, G.IsLink e x y := by
+--   simp only [Inc, sInter_isLink]
+
+-- @[simp]
+-- lemma sInter_isLoopAt_iff {s : Set (Graph α β)} (hs : s.Nonempty) :
+--     (Graph.sInter s hs).IsLoopAt e x ↔ ∀ G ∈ s, G.IsLoopAt e x := by
+--   simp only [IsLoopAt, sInter_isLink]
+
+-- @[simp]
+-- lemma sInter_isNonloopAt_iff {s : Set (Graph α β)} (hs : s.Nonempty) :
+--     (Graph.sInter s hs).IsNonloopAt e x ↔ ∃ y ≠ x, ∀ G ∈ s, G.IsLink e x y := by
+--   simp only [IsNonloopAt, sInter_isLink]
+
+-- @[simp]
+-- lemma induce_sInter {s : Set (Graph α β)} (hs : s.Nonempty) (X : Set α) :
+--     (Graph.sInter s hs)[X] = .sInter ((·[X]) '' s) (by simpa) := by
+--   refine Graph.ext (by simp; exact (biInter_const hs X).symm) fun e x y ↦ ?_
+--   simp +contextual only [induce_isLink_iff, sInter_isLink, mem_image, forall_exists_index, and_imp,
+--     forall_apply_eq_imp_iff₂, iff_def, and_self, implies_true, true_and]
+--   exact fun h ↦ (h _ hs.some_mem).right
+
+-- @[simp]
+-- lemma vertexDelete_sInter {s : Set (Graph α β)} (hs : s.Nonempty) (X : Set α) :
+--     (Graph.sInter s hs) - X = .sInter ((· - X) '' s) (by simpa) := by
+--   refine Graph.ext (by simp [biInter_diff_distrib hs]) fun e x y ↦ ?_
+--   simp +contextual only [vertexDelete_isLink_iff, sInter_isLink, mem_image, forall_exists_index,
+--     and_imp, forall_apply_eq_imp_iff₂, iff_def, not_false_eq_true, and_self, implies_true, true_and]
+--   exact fun h ↦ (h _ hs.some_mem).right
+
+-- @[simp]
+-- lemma edgeDelete_sInter {s : Set (Graph α β)} (hs : s.Nonempty) (F : Set β) :
+--     (Graph.sInter s hs) ＼ F = .sInter ((· ＼ F) '' s) (by simpa) :=
+--   Graph.ext (by simp [biInter_diff_distrib hs]) fun e x y ↦ by
+--   simp +contextual only [edgeDelete_isLink, sInter_isLink, mem_image, forall_exists_index, and_imp,
+--     forall_apply_eq_imp_iff₂, iff_def, not_false_eq_true, and_self, implies_true, true_and]
+--   exact fun h ↦ (h _ hs.some_mem).right
+
+-- @[simp]
+-- lemma edgeRestrict_sInter {s : Set (Graph α β)} (hs : s.Nonempty) (F : Set β) :
+--     (Graph.sInter s hs) ↾ F = .sInter ((· ↾ F) '' s) (by simpa) :=
+--   Graph.ext (by simp [biInter_diff_distrib hs]) fun e x y ↦ by
+--   simp +contextual only [edgeRestrict_isLink, sInter_isLink, mem_image, forall_exists_index,
+--     and_imp, forall_apply_eq_imp_iff₂, iff_def, and_self, implies_true, and_true, true_and]
+--   exact fun h ↦ (h _ hs.some_mem).left
+
+-- /-! ### Intersections -/
+
+-- /-- The intersection of two graphs `G` and `H`. There seems to be no good way to
+-- defined junk values so that this has the right edge and vertex set, so the
+-- edges are precisely those on which `G` and `H` agree, and the edge set is a subset
+-- of `E(G) ∩ E(H)`,
+-- with equality if `G` and `H` are compatible.   -/
+-- protected def inter (G H : Graph α β) : Graph α β where
+--   vertexSet := V(G) ∩ V(H)
+--   IsLink e x y := G.IsLink e x y ∧ H.IsLink e x y
+--   isLink_symm _ _ _ _ h := ⟨h.1.symm, h.2.symm⟩
+--   dup_or_dup_of_isLink_of_isLink _ _ _ _ _ h h' := h.1.left_eq_or_eq h'.1
+--   edge_mem_iff_exists_isLink e := by simp
+--   left_mem_of_isLink e x y h := ⟨h.1.left_mem, h.2.left_mem⟩
+
+-- instance : Inter (Graph α β) where inter := Graph.inter
+
+-- @[simp]
+-- lemma inter_vertexSet (G H : Graph α β) : V(G ∩ H) = V(G) ∩ V(H) := rfl
+
+-- @[simp]
+-- lemma inter_isLink_iff : (G ∩ H).IsLink e x y ↔ G.IsLink e x y ∧ H.IsLink e x y := Iff.rfl
+
+-- protected lemma inter_comm (G H : Graph α β) : G ∩ H = H ∩ G :=
+--   Graph.ext (Set.inter_comm ..) <| by simp [and_comm]
+
+-- lemma inter_edgeSet (G H : Graph α β) :
+--     E(G ∩ H) = {e ∈ E(G) ∩ E(H) | G.IsLink e = H.IsLink e} := by
+--   simp only [edgeSet_eq_setOf_exists_isLink, inter_isLink_iff, mem_inter_iff, mem_setOf_eq,
+--     funext_iff, eq_iff_iff, Set.ext_iff]
+--   exact fun e ↦ ⟨fun ⟨x, y, hfG, hfH⟩ ↦ ⟨⟨⟨_, _, hfG⟩, ⟨_, _, hfH⟩⟩,
+--     fun z w ↦ by rw [hfG.isLink_iff_sym2_eq, hfH.isLink_iff_sym2_eq]⟩,
+--     fun ⟨⟨⟨x, y, hexy⟩, ⟨z, w, hezw⟩⟩, h⟩ ↦ ⟨x, y, hexy, by rwa [← h]⟩⟩
+
+-- lemma inter_edgeSet_subset : E(G ∩ H) ⊆ E(G) ∩ E(H) := by
+--   simp +contextual [inter_edgeSet, subset_def]
+
+-- @[simp]
+-- lemma inter_inc_iff : (G ∩ H).Inc e x ↔ ∃ y, G.IsLink e x y ∧ H.IsLink e x y := by
+--   simp [Inc]
+
+-- @[simp]
+-- lemma inter_isLoopAt_iff : (G ∩ H).IsLoopAt e x ↔ G.IsLoopAt e x ∧ H.IsLoopAt e x := by
+--   simp [← isLink_self_iff]
+
+-- @[simp]
+-- lemma inter_isNonloopAt_iff :
+--     (G ∩ H).IsNonloopAt e x ↔ ∃ y ≠ x, G.IsLink e x y ∧ H.IsLink e x y := by
+--   simp [IsNonloopAt]
+
+-- @[simp]
+-- protected lemma inter_le_left : G ∩ H ≤ G where
+--   vertex_subset := inter_subset_left
+--   isLink_of_isLink := by simp +contextual
+
+-- @[simp]
+-- protected lemma inter_le_right : G ∩ H ≤ H :=
+--   Graph.inter_comm _ _ ▸ Graph.inter_le_left
+
+-- protected lemma le_inter (h₁ : H ≤ G₁) (h₂ : H ≤ G₂) : H ≤ G₁ ∩ G₂ where
+--   vertex_subset := subset_inter (vertexSet_mono h₁) (vertexSet_mono h₂)
+--   isLink_of_isLink e x y h := by simp [h.of_le h₁, h.of_le h₂]
+
+-- instance : SemilatticeInf (Graph α β) where
+--   inf := Graph.inter
+--   inf_le_left _ _ := Graph.inter_le_left
+--   inf_le_right _ _ := Graph.inter_le_right
+--   le_inf _ _ _ := Graph.le_inter
+
+-- @[simp]
+-- lemma inf_eq_inter : H₁ ⊓ H₂ = H₁ ∩ H₂ := rfl
+
+-- @[simp]
+-- lemma inter_eq_bot_iff : H₁ ∩ H₂ = ⊥ ↔ V(H₁) ∩ V(H₂) = ∅ := by
+--   rw [← vertexSet_eq_empty_iff, inter_vertexSet]
+
+-- lemma disjoint_iff_inter_eq_bot : Disjoint H₁ H₂ ↔ H₁ ∩ H₂ = ⊥ := by
+--   rw [disjoint_iff, inf_eq_inter]
+
+-- @[simp]
+-- lemma disjoint_iff_vertexSet_inter_eq_empty : Disjoint H₁ H₂ ↔ V(H₁) ∩ V(H₂) = ∅ := by
+--   rw [disjoint_iff_inter_eq_bot, inter_eq_bot_iff]
+
+-- lemma disjoint_iff_vertexSet_disjoint : Disjoint H₁ H₂ ↔ Disjoint V(H₁) V(H₂) := by
+--   rw [disjoint_iff_inter_eq_bot, inter_eq_bot_iff, Set.disjoint_iff_inter_eq_empty]
+
+-- alias ⟨Disjoint.vertex_disjoint, _⟩ := disjoint_iff_vertexSet_disjoint
+
+-- lemma Compatible.inter_edgeSet (h : G.Compatible H) : E(G ∩ H) = E(G) ∩ E(H) := by
+--   rw [Graph.inter_edgeSet]
+--   exact le_antisymm (fun e he ↦ he.1) fun e he ↦ ⟨he, h he⟩
+
+-- lemma inter_eq_iInter : G ∩ H = Graph.iInter (fun b ↦ bif b then G else H) :=
+--   Graph.ext (by simp [Set.inter_eq_iInter, Bool.apply_cond]) (by simp [and_comm])
+
+-- lemma le_inter_iff : H ≤ G₁ ∩ G₂ ↔ H ≤ G₁ ∧ H ≤ G₂ := by
+--   simp [inter_eq_iInter, and_comm]
+
+-- lemma inter_eq_self_of_le (hle : G ≤ H) : G ∩ H = G :=
+--   le_antisymm Graph.inter_le_left <| by simpa [le_inter_iff]
+
+-- lemma le_of_inter_eq_self (h : G ∩ H = G) : G ≤ H := by
+--   rw [← h]
+--   exact Graph.inter_le_right
+
+-- lemma inter_mono_left (hle : G₁ ≤ G₂) : G₁ ∩ H ≤ G₂ ∩ H := by
+--   rw [le_inter_iff]
+--   exact ⟨Graph.inter_le_left.trans hle, Graph.inter_le_right⟩
+
+-- lemma inter_mono_right (hle : H₁ ≤ H₂) : G ∩ H₁ ≤ G ∩ H₂ := by
+--   rw [le_inter_iff]
+--   exact ⟨Graph.inter_le_left, Graph.inter_le_right.trans hle⟩
+
+-- lemma inter_mono (hleG : G₁ ≤ G₂) (hleH : H₁ ≤ H₂) : G₁ ∩ H₁ ≤ G₂ ∩ H₂ :=
+--   (inter_mono_right hleH).trans (inter_mono_left hleG)
+
+-- lemma stronglyDisjoint_iff_disjoint_of_compatible (h : H₁.Compatible H₂) :
+--     StronglyDisjoint H₁ H₂ ↔ Disjoint H₁ H₂ := by
+--   rw [stronglyDisjoint_iff_vertexSet_disjoint_compatible, Set.disjoint_iff_inter_eq_empty,
+--     disjoint_iff, ← vertexSet_eq_empty_iff]
+--   simp [h]
+
+-- lemma edgeSet_induce_inter_eq_edgeSet_induce_of_le (h : G ≤ H) : E(G) ∩ E(H[X]) = E(G[X]) :=
+--   Set.ext fun _ ↦ ⟨fun ⟨he, x, y, hl, hx, hy⟩ => ⟨x, y, hl.of_le_of_mem h he, hx, hy⟩,
+--     fun ⟨x, y, hl, hx, hy⟩ => ⟨hl.edge_mem, x, y, hl.of_le h, hx, hy⟩⟩
+
+-- lemma induce_inter (X Y : Set α) : G[X ∩ Y] = G[X] ∩ G[Y] :=
+--   Graph.ext (by simp) fun e x y ↦ by
+--   simp +contextual only [induce_isLink_iff, mem_inter_iff, inter_isLink_iff, iff_def, and_self,
+--     implies_true]
+
+-- lemma induce_inter_distrib (X : Set α) : (G ∩ H)[X] = G[X] ∩ H[X] :=
+--   Graph.ext (by simp) fun e x y ↦ by
+--   simp +contextual only [induce_isLink_iff, inter_isLink_iff, iff_def, and_self, implies_true]
+
+-- lemma vertexDelete_union (X Y : Set α) : G - (X ∪ Y) = (G - X) ∩ (G - Y) :=
+--   Graph.ext (by simp [diff_inter_diff]) fun e x y ↦ by
+--   simp +contextual only [vertexDelete_isLink_iff, mem_union, not_or, inter_isLink_iff, iff_def,
+--     not_false_eq_true, and_self, implies_true]
+
+-- lemma vertexDelete_inter_distrib (X : Set α) : (G ∩ H) - X = (G - X) ∩ (H - X) :=
+--   Graph.ext (by simp [diff_inter_distrib_right]) fun e x y ↦ by
+--   simp +contextual only [vertexDelete_isLink_iff, inter_isLink_iff, iff_def, not_false_eq_true,
+--     and_self, implies_true]
+
+-- lemma edgeDelete_union (F₁ F₂ : Set β) : G ＼ (F₁ ∪ F₂) = (G ＼ F₁) ∩ (G ＼ F₂) :=
+--   Graph.ext (by simp [diff_inter_diff]) fun e x y ↦ by
+--   simp +contextual only [edgeDelete_isLink, mem_union, not_or, inter_isLink_iff, iff_def,
+--     not_false_eq_true, and_self, implies_true]
+
+-- lemma edgeDelete_inter_distrib (F : Set β) : (G ∩ H) ＼ F = (G ＼ F) ∩ (H ＼ F) :=
+--   Graph.ext (by simp) fun e x y ↦ by
+--   simp +contextual only [edgeDelete_isLink, inter_isLink_iff, iff_def, not_false_eq_true, and_self,
+--     implies_true]
+
+-- lemma edgeRestrict_inter (F₁ F₂ : Set β) : (G ↾ (F₁ ∩ F₂)) = (G ↾ F₁) ∩ (G ↾ F₂) :=
+--   Graph.ext (by simp) fun e x y ↦ by
+--   simp +contextual only [edgeRestrict_isLink, mem_inter_iff, inter_isLink_iff, iff_def, and_self,
+--     implies_true]
+
+-- lemma edgeRestrict_inter_distrib (F : Set β) : (G ∩ H) ↾ F = (G ↾ F) ∩ (H ↾ F) :=
+--   Graph.ext (by simp) fun e x y ↦ by
+--   simp +contextual only [edgeRestrict_isLink, inter_isLink_iff, iff_def, and_self, implies_true]
+
+-- protected lemma inter_distrib_iInter [Nonempty ι] {H : ι → Graph α β} :
+--     G ∩ (Graph.iInter H) = Graph.iInter (fun i ↦ G ∩ (H i)) :=
+--   Graph.ext (by simp [inter_iInter]) (by
+--     simp only [inter_isLink_iff, iInter_isLink]
+--     rintro i x y
+--     rw [forall_and_left])
+
+-- protected lemma inter_distrib_sInter [Nonempty ι] {s : Set (Graph α β)} (hne : s.Nonempty) :
+--     G ∩ (Graph.sInter s hne) = Graph.sInter ((G ∩ ·) '' s) (by simpa) := by
+--   rw [Graph.sInter_image hne]
+--   unfold Graph.sInter
+--   have := hne.to_subtype
+--   rw [Graph.inter_distrib_iInter]
+
+-- protected lemma inter_distrib_iUnion {H : ι → Graph α β} (hH : Pairwise (Compatible on H)) :
+--     G ∩ (Graph.iUnion H hH) = Graph.iUnion (fun i ↦ G ∩ (H i))
+--       (fun _ _ hne ↦ (hH hne).mono Graph.inter_le_right Graph.inter_le_right) :=
+--   Graph.ext (by simp [inter_iUnion]) (by simp)
+
+-- protected lemma inter_distrib_sUnion (hs : s.Pairwise Compatible) :
+--     G ∩ (Graph.sUnion s hs) = Graph.sUnion ((fun K ↦ G ∩ K) '' s) (by
+--       rintro _ ⟨K₁, hK₁, rfl⟩ _ ⟨K₂, hK₂, rfl⟩ -
+--       exact (hs.of_refl hK₁ hK₂).mono Graph.inter_le_right Graph.inter_le_right) := by
+--   ext <;> aesop
+
+-- lemma Pairwise.union_compatible {s t : Set (Graph α β)} (hst : (s ∪ t).Pairwise Compatible) :
+--     (Graph.sUnion s (hst.mono subset_union_left)).Compatible
+--     (Graph.sUnion t (hst.mono subset_union_right)) := by
+--   refine compatible_of_le_le (G := Graph.sUnion (s ∪ t) hst) ?_ ?_ <;> rw [Graph.sUnion_le_iff]
+--   <;> exact fun G hG ↦ Graph.le_sUnion hst (by simp [hG])
+
+-- lemma sUnion_union_sUnion {s t : Set (Graph α β)} (hst : (s ∪ t).Pairwise Compatible) :
+--     Graph.sUnion s (hst.mono subset_union_left) ∪ Graph.sUnion t (hst.mono subset_union_right) =
+--     Graph.sUnion (s ∪ t) hst := by
+--   have hs : s.Pairwise Compatible := hst.mono subset_union_left
+--   have ht : t.Pairwise Compatible := hst.mono subset_union_right
+--   refine Graph.ext (by aesop) fun e x y ↦ ?_
+--   rw [(Pairwise.union_compatible hst).union_isLink_iff]
+--   aesop
+
+-- protected lemma sInter_inter_sInter {s t : Set (Graph α β)} (hs : s.Nonempty) (ht : t.Nonempty) :
+--     Graph.sInter s hs ∩ .sInter t ht = .sInter (s ∪ t) (by simp [hs]) := by
+--   ext <;> aesop
+
+-- lemma Compatible.sum_compatible {G : ι → Graph α β} {H : ι' → Graph α β}
+--     (hGH : Pairwise (Compatible on (Sum.elim G H))) :
+--     (Graph.iUnion G (hGH.sum_left)).Compatible (Graph.iUnion H (hGH.sum_right)) :=
+--   compatible_of_le_le (iUnion_left_le_iUnion_sum hGH) <| iUnion_right_le_iUnion_sum hGH
+
+-- protected lemma iUnion_sum [Nonempty ι] [Nonempty ι'] {G : ι → Graph α β}
+--     {H : ι' → Graph α β} (hGH : Pairwise (Compatible on (Sum.elim G H))) :
+--     Graph.iUnion (Sum.elim G H) hGH = (.iUnion G hGH.sum_left) ∪ (.iUnion H hGH.sum_right) := by
+--   refine le_antisymm ?_ <| Graph.union_le (iUnion_left_le_iUnion_sum hGH)
+--     (iUnion_right_le_iUnion_sum hGH)
+--   rw [Graph.iUnion_le_iff]
+--   rintro (i | i) <;> simp only [Sum.elim_inl, Sum.elim_inr]
+--   · exact le_trans (Graph.le_iUnion hGH.sum_left i) (Graph.left_le_union _ _)
+--   · exact le_trans (Graph.le_iUnion hGH.sum_right i)
+--       (Compatible.right_le_union (Compatible.sum_compatible hGH))
+
+-- protected lemma iInter_sum [Nonempty ι] [Nonempty ι'] {G : ι → Graph α β}
+--     {H : ι' → Graph α β} : Graph.iInter (Sum.elim G H) = .iInter G ∩ .iInter H := by
+--   ext <;> aesop
+
+-- protected lemma iInter_option [Nonempty ι] {G₁ : Graph α β} {G : ι → Graph α β} :
+--     Graph.iInter (Option.elim · G₁ G) = G₁ ∩ Graph.iInter G :=
+--   Graph.ext (by simp [Set.iInter_option]) (by simp [Option.forall])
+
+-- protected lemma sInter_insert {s : Set (Graph α β)} (G : Graph α β) (hne : s.Nonempty) :
+--     Graph.sInter (insert G s) (by simp) = G ∩ Graph.sInter s hne := by
+--   ext v <;> simp
+
+-- lemma iInter_option_eq_sInter_insert {G₁ : Graph α β} {G : ι → Graph α β} :
+--     Graph.iInter (Option.elim · G₁ G) = Graph.sInter (insert G₁ (range G)) (by simp) := by
+--   obtain hι | hι := isEmpty_or_nonempty ι
+--   · simp [range_eq_empty G]
+--   rw [Graph.sInter_insert _ (range_nonempty _), Graph.sInter_range, Graph.iInter_option]
+
+-- -- protected lemma union_iInter [Nonempty ι] {H : ι → Graph α β} (hc : ∀ i, G.Compatible (H i))
+-- --     (hH : Pairwise (Compatible on H)) :
+-- --     G ∪ (Graph.iInter H hH) = Graph.iInter (fun i ↦ G ∪ (H i))
+-- --     (by
+-- --       refine fun i j hij ↦ (h)
+-- --     )
+
+-- --     := by
+-- --   _
+
+--   -- rw [Graph.sUnion, Graph.sUnion]
+--   -- generalize_proofs h₁ h₂
+--   -- rw [Graph.inter_distrib_iUnion _]
+
+
+
+
+
+-- section Subgraph
+
+-- /-! ### Subgraphs -/
+
+-- variable {H : ι → Graph α β} {H₁ H₂ : Graph α β}
+
+-- lemma pairwise_compatible_of_subgraph {H : ι → Graph α β} (h : ∀ i, H i ≤ G) :
+--     Pairwise (Compatible on H) :=
+--   fun i j _ ↦ compatible_of_le_le (h i) (h j)
+
+-- lemma set_pairwise_compatible_of_subgraph (h : ∀ ⦃H⦄, H ∈ s → H ≤ G) :
+--     s.Pairwise Compatible :=
+--   fun _ hi _ hj _ ↦ compatible_of_le_le (h hi) (h hj)
+
+-- protected lemma iUnion_le_of_forall_le (h : ∀ i, H i ≤ G) :
+--     Graph.iUnion H (pairwise_compatible_of_subgraph h) ≤ G := by
+--   simpa
+
+-- protected lemma sUnion_le_of_forall_le (h : ∀ ⦃H⦄, H ∈ s → H ≤ G) :
+--     Graph.sUnion s (set_pairwise_compatible_of_subgraph h) ≤ G := by
+--   simpa
+
+-- protected lemma iInter_le_of_forall_le [Nonempty ι] (h : ∀ i, H i ≤ G) :
+--     Graph.iInter H ≤ G :=
+--   (Graph.iInter_le (Classical.arbitrary ι)).trans <| h _
+
+-- protected lemma sInter_le_of_forall_le (h : ∀ ⦃H⦄, H ∈ s → H ≤ G) (hne : s.Nonempty) :
+--     Graph.sInter s hne ≤ G :=
+--   have := hne.to_subtype
+--   Graph.iInter_le_of_forall_le (by simpa)
+
+-- /-- A union of closed subgraphs of `G` is a closed subgraph of `G`. -/
+-- lemma iUnion_isClosedSubgraph (h : ∀ i, H i ≤c G) :
+--     Graph.iUnion H (pairwise_compatible_of_subgraph (fun i ↦ (h i).le)) ≤c G where
+--   le := Graph.iUnion_le_of_forall_le fun i ↦ (h i).le
+--   closed e x he := by
+--     simp only [iUnion_vertexSet, mem_iUnion, iUnion_edgeSet, forall_exists_index]
+--     exact fun i hxi ↦ ⟨_, (he.of_isClosedSubgraph_of_mem (h i) hxi).edge_mem⟩
+
+-- /-- A nonempty union of spanning subgraphs of `G` is a spanning subgraph of `G`. -/
+-- lemma iUnion_isSpanningSubgraph [Nonempty ι] (h : ∀ i, H i ≤s G) :
+--     Graph.iUnion H (pairwise_compatible_of_subgraph (fun i ↦ (h i).le)) ≤s G where
+--   le := Graph.iUnion_le_of_forall_le fun i ↦ (h i).le
+--   vertexSet_eq := by simp [(h _).vertexSet_eq, iUnion_const]
+
+-- -- A weakening of the previous lemma.
+-- lemma iUnion_isSpanningSubgraph_of_exists_isSpanningSubgraph_of_forall_le [Nonempty ι]
+--     (h : ∀ i, H i ≤ G) (hH : ∃ i, H i ≤s G) :
+--     Graph.iUnion H (pairwise_compatible_of_subgraph h) ≤s G where
+--   le := Graph.iUnion_le_of_forall_le h
+--   vertexSet_eq := by
+--     apply le_antisymm
+--     · simp only [iUnion_vertexSet, le_eq_subset, iUnion_subset_iff]
+--       exact fun i ↦ (h i).vertex_subset
+--     obtain ⟨i, hi⟩ := hH
+--     rw [← hi.vertexSet_eq]
+--     exact subset_iUnion_of_subset i fun ⦃a⦄ a ↦ a
+
+-- /-- A nonempty intersection of induced subgraphs `G` is an induced subgraph of `G`-/
+-- lemma iInter_isInducedSubgraph [Nonempty ι] (h : ∀ i, H i ≤i G) :
+--     Graph.iInter H ≤i G where
+--   le := Graph.iInter_le_of_forall_le fun i ↦ (h i).le
+--   isLink_of_mem_mem := by
+--     simp only [iInter_vertexSet, mem_iInter, iInter_isLink]
+--     exact fun e x y he hx hy i ↦ (h i).isLink_of_mem_mem he (hx i) (hy i)
+
+-- /-- A nonempty intersection of spanning subgraphs of `G` is a spanning subgraph of `G`.-/
+-- lemma iInter_isSpanningSubgraph [Nonempty ι] (h : ∀ i, H i ≤s G) :
+--     Graph.iInter H ≤s G where
+--   le := Graph.iInter_le_of_forall_le fun i ↦ (h i).le
+--   vertexSet_eq := iInter_eq_const fun i ↦ (h i).vertexSet_eq
+
+-- /-- A nonempty intersection of closed subgraphs `G` is an induced subgraph of `G`-/
+-- lemma iInter_isClosedSubgraph [Nonempty ι] (h : ∀ i, H i ≤c G) :
+--     Graph.iInter H ≤c G where
+--   le := Graph.iInter_le_of_forall_le fun i ↦ (h i).le
+--   closed e x he := by
+--     simp only [iInter_vertexSet, mem_iInter, iInter_edgeSet, mem_setOf_eq]
+--     rintro hx
+--     obtain ⟨y, hy⟩ := he
+--     use x, y, fun i ↦ by rwa [(h i).isLink_iff_of_mem (hx i)]
+
+-- lemma sUnion_isClosedSubgraph (hs : ∀ ⦃H⦄, H ∈ s → H ≤c G) :
+--     Graph.sUnion s (set_pairwise_compatible_of_subgraph (fun _ h ↦ (hs h).le)) ≤c G :=
+--   iUnion_isClosedSubgraph <| by simpa
+
+-- lemma sUnion_isSpanningSubgraph (hs : ∀ ⦃H⦄, H ∈ s → H ≤s G) (hne : s.Nonempty) :
+--     Graph.sUnion s (set_pairwise_compatible_of_subgraph (fun _ h ↦ (hs h).le)) ≤s G :=
+--   have := hne.to_subtype
+--   iUnion_isSpanningSubgraph <| by simpa
+
+-- lemma sInter_isInducedSubgraph (hs : ∀ ⦃H⦄, H ∈ s → H ≤i G) (hne : s.Nonempty) :
+--     Graph.sInter s hne ≤i G :=
+--   have := hne.to_subtype
+--   iInter_isInducedSubgraph <| by simpa
+
+-- lemma sInter_isClosedSubgraph (hs : ∀ ⦃H⦄, H ∈ s → H ≤c G) (hne : s.Nonempty) :
+--     Graph.sInter s hne ≤c G :=
+--   have := hne.to_subtype
+--   iInter_isClosedSubgraph <| by simpa
+
+-- lemma isClosedSubgraph_iUnion_of_stronglyDisjoint (h : Pairwise (StronglyDisjoint on H)) (i : ι) :
+--     H i ≤c Graph.iUnion H (h.mono fun _ _ ↦ StronglyDisjoint.compatible) where
+--   le := Graph.le_iUnion ..
+--   closed e x he hx := by
+--     obtain ⟨j, hj : (H j).Inc e x⟩ := (iUnion_inc_iff ..).1 he
+--     obtain rfl | hne := eq_or_ne i j
+--     · exact hj.edge_mem
+--     exact False.elim <| (h hne).vertex.notMem_of_mem_left hx hj.vertex_mem
+
+-- lemma isClosedSubgraph_sUnion_of_stronglyDisjoint (s : Set (Graph α β))
+--     (hs : s.Pairwise StronglyDisjoint) (hG : G ∈ s) : G ≤c Graph.sUnion s (hs.mono' (by simp)) :=
+--   isClosedSubgraph_iUnion_of_stronglyDisjoint ((pairwise_subtype_iff_pairwise_set ..).2 hs) ⟨G, hG⟩
+
+-- lemma isClosedSubgraph_union_left_of_vertexSet_disjoint (h : Disjoint V(H₁) V(H₂)) :
+--     H₁ ≤c H₁ ∪ H₂ := by
+--   refine ⟨Graph.left_le_union H₁ H₂, fun e x hinc hx₁ => ?_⟩
+--   have hninc : ¬ H₂.Inc e x := fun hinc ↦ h.notMem_of_mem_left hx₁ hinc.vertex_mem
+--   simp only [union_inc_iff, hninc, false_and, or_false] at hinc
+--   exact hinc.edge_mem
+
+-- lemma Disjoint.isClosedSubgraph_union_left (h : Disjoint H₁ H₂) : H₁ ≤c H₁ ∪ H₂ :=
+--   isClosedSubgraph_union_left_of_vertexSet_disjoint <| Disjoint.vertex_disjoint h
+
+-- lemma StronglyDisjoint.isClosedSubgraph_union_left (h : StronglyDisjoint H₁ H₂) :
+--     H₁ ≤c H₁ ∪ H₂ := by
+--   rw [(stronglyDisjoint_le_compatible _ _ h).union_eq_sUnion]
+--   exact isClosedSubgraph_sUnion_of_stronglyDisjoint _ (by simp [Set.Pairwise, h, h.symm]) (by simp)
+
+-- lemma StronglyDisjoint.isClosedSubgraph_union_right (h : StronglyDisjoint H₁ H₂) :
+--     H₂ ≤c H₁ ∪ H₂ := by
+--   rw [(stronglyDisjoint_le_compatible _ _ h).union_eq_sUnion]
+--   exact isClosedSubgraph_sUnion_of_stronglyDisjoint _ (by simp [Set.Pairwise, h, h.symm]) (by simp)
+
+-- lemma IsClosedSubgraph.union (h₁ : H₁ ≤c G) (h₂ : H₂ ≤c G) : H₁ ∪ H₂ ≤c G := by
+--   rw [(compatible_of_le_le h₁.le h₂.le).union_eq_iUnion]
+--   exact iUnion_isClosedSubgraph <| by simp [h₁,h₂]
+
+-- lemma IsSpanningSubgraph.union (h₁ : H₁ ≤s G) (h₂ : H₂ ≤s G) : H₁ ∪ H₂ ≤s G := by
+--   rw [(compatible_of_le_le h₁.le h₂.le).union_eq_iUnion]
+--   exact iUnion_isSpanningSubgraph <| by simp [h₁,h₂]
+
+-- lemma IsSpanningSubgraph.union_left (h₁ : H₁ ≤s G) (h₂ : H₂ ≤ G) : H₁ ∪ H₂ ≤s G := by
+--   rw [(compatible_of_le_le h₁.le h₂).union_eq_iUnion]
+--   exact iUnion_isSpanningSubgraph_of_exists_isSpanningSubgraph_of_forall_le (by simp [h₁.le, h₂])
+--     ⟨True, h₁⟩
+
+-- lemma IsSpanningSubgraph.union_right (h₁ : H₁ ≤ G) (h₂ : H₂ ≤s G) : H₁ ∪ H₂ ≤s G := by
+--   rw [(compatible_of_le_le h₁ h₂.le).union_eq_iUnion]
+--   exact iUnion_isSpanningSubgraph_of_exists_isSpanningSubgraph_of_forall_le (by simp [h₁, h₂.le])
+--     ⟨False, h₂⟩
+
+-- lemma IsInducedSubgraph.inter (h₁ : H₁ ≤i G) (h₂ : H₂ ≤i G) : H₁ ∩ H₂ ≤i G := by
+--   rw [inter_eq_iInter]
+--   exact iInter_isInducedSubgraph <| by simp [h₁,h₂]
+
+-- lemma IsClosedSubgraph.inter (h₁ : H₁ ≤c G) (h₂ : H₂ ≤c G) : H₁ ∩ H₂ ≤c G := by
+--   rw [inter_eq_iInter]
+--   exact iInter_isClosedSubgraph <| by simp [h₁,h₂]
+
+-- lemma IsClosedSubgraph.inter_le {K G H : Graph α β} (hKG : K ≤c G) (hle : H ≤ G) : K ∩ H ≤c H where
+--   le := Graph.inter_le_right
+--   closed e x hex hx := by
+--     rw [inter_vertexSet] at hx
+--     have heK := ((hex.of_le hle).of_isClosedSubgraph_of_mem hKG hx.1).edge_mem
+--     rw [(compatible_of_le_le hKG.le hle).inter_edgeSet]
+--     exact ⟨heK, hex.edge_mem⟩
+
+-- @[simp]
+-- lemma le_bot_iff : G ≤ ⊥ ↔ G = ⊥ := _root_.le_bot_iff
+
+-- @[simp]
+-- lemma isClosedSubgraph_bot_iff : G ≤c ⊥ ↔ G = ⊥ :=
+--   ⟨fun h => le_bot_iff.mp h.le, fun h => h ▸ bot_isClosedSubgraph ⊥⟩
+
+-- @[simp]
+-- lemma isSpanningSubgraph_bot_iff : G ≤s ⊥ ↔ G = ⊥ :=
+--   ⟨fun h => le_bot_iff.mp h.le, fun h => h ▸ ⟨le_rfl, rfl⟩⟩
+
+-- @[simp]
+-- lemma isInducedSubgraph_bot_iff : G ≤i ⊥ ↔ G = ⊥ :=
+--   ⟨fun h => le_bot_iff.mp h.le, fun h => h ▸ bot_isInducedSubgraph ⊥⟩
+
+-- @[simp]
+-- lemma induce_empty : G[∅] = ⊥ := by
+--   rw [← vertexSet_eq_empty_iff, induce_vertexSet]
+
+-- end Subgraph
+
+-- /-! ### Adding one edge -/
+
+-- @[simp]
+-- lemma singleEdge_compatible_iff :
+--     Compatible (Graph.singleEdge u v e) G ↔ (e ∈ E(G) → G.IsLink e u v) := by
+--   refine ⟨fun h he ↦ by simp [← h ⟨by simp, he⟩], fun h f ⟨hfe, hf⟩ ↦ ?_⟩
+--   obtain rfl : f = e := by simpa using hfe
+--   ext x y
+--   simp only [singleEdge_isLink, (h hf).isLink_iff]
+--   tauto
+
+-- /-- Add a new edge `e` between vertices `a` and `b`. If `e` is already in the graph,
+-- its ends change to `a` and `b`. -/
+-- @[simps! edgeSet vertexSet]
+-- protected def addEdge (G : Graph α β) (e : β) (a b : α) : Graph α β :=
+--   Graph.singleEdge a b e ∪ G
+
+-- lemma addEdge_isLink (G : Graph α β) (e : β) (a b : α) : (G.addEdge e a b).IsLink e a b := by
+--   simp [Graph.addEdge, union_isLink_iff]
+
+-- lemma addEdge_isLink_of_ne (hf : G.IsLink f x y) (hne : f ≠ e) (a b : α) :
+--     (G.addEdge e a b).IsLink f x y := by
+--   simpa [Graph.addEdge, union_isLink_iff, hne]
+
+-- lemma addEdge_isLink_iff {a b : α} (he : e ∉ E(G)) :
+--     (G.addEdge e a b).IsLink f x y ↔ (f = e ∧ s(a,b) = s(x,y)) ∨ G.IsLink f x y := by
+--   have hc : Compatible (Graph.singleEdge x y e) G := by simp [he]
+--   simp only [Graph.addEdge, union_isLink_iff, singleEdge_isLink, singleEdge_edgeSet,
+--     mem_singleton_iff, edgeDelete_isLink, Sym2.eq, Sym2.rel_iff', Prod.mk.injEq, Prod.swap_prod_mk]
+--   obtain rfl | hne := eq_or_ne e f
+--   · have hl : ¬ G.IsLink e x y := fun h ↦ he h.edge_mem
+--     simp only [true_and, not_true_eq_false, hl, and_self, or_false]
+--     tauto
+--   simp [hne.symm]
+
+-- lemma addEdge_deleteEdge (he : e ∉ E(G)) (hx : x ∈ V(G)) (hy : y ∈ V(G)) :
+--     (G.addEdge e x y) ＼ {e} = G := by
+--   have hc : Compatible (Graph.singleEdge x y e) G := by simp [he]
+--   simp only [Graph.addEdge, Graph.ext_iff, edgeDelete_vertexSet, union_vertexSet,
+--     singleEdge_vertexSet, union_eq_right, insert_subset_iff, hx, singleton_subset_iff, hy, and_self,
+--     edgeDelete_isLink, hc.union_isLink_iff, singleEdge_isLink, mem_singleton_iff, true_and]
+--   intro f p q
+--   obtain rfl | hne := eq_or_ne f e
+--   · suffices ¬ G.IsLink f p q by simpa
+--     exact fun hf ↦ he hf.edge_mem
+--   simp [hne]
+
+-- lemma addEdge_le (hle : H ≤ G) (he : G.IsLink e x y) : H.addEdge e x y ≤ G :=
+--   Graph.union_le (by simpa) hle
+
+-- lemma le_addEdge (he : e ∉ E(G)) : G ≤ G.addEdge e x y :=
+--   Compatible.right_le_union <| by simp [he]
+
+-- lemma addEdge_mono (hle : H ≤ G) : H.addEdge e x y ≤ G.addEdge e x y :=
+--   union_mono_right hle
+
+-- lemma deleteEdge_le_addEdge : G ＼ {e} ≤ G.addEdge e x y := by
+--   rw [Graph.addEdge, union_eq_union_edgeDelete]
+--   simp only [singleEdge_edgeSet]
+--   exact Compatible.right_le_union <| by simp
+
+-- lemma deleteEdge_addEdge : (G ＼ {e}).addEdge e x y = G.addEdge e x y := by
+--   refine le_antisymm (addEdge_mono edgeDelete_le) ?_
+--   unfold Graph.addEdge
+--   rw [union_le_iff]
+--   refine ⟨Graph.left_le_union (Graph.singleEdge x y e) (G ＼ {e}), Compatible.right_le_union ?_⟩
+--   simp
+
+-- lemma addEdge_eq_self (hbtw : G.IsLink e x y) : G.addEdge e x y = G :=
+--   le_antisymm (addEdge_le (by simp) hbtw) <| Compatible.right_le_union <| by simp [hbtw]
+
+-- lemma addEdge_idem : (G.addEdge e x y).addEdge e x y = G.addEdge e x y :=
+--   addEdge_eq_self <| addEdge_isLink G e x y
+
+-- lemma isSpanningSubgraph_addEdge (he : e ∉ E(G)) (hx : x ∈ V(G)) (hy : y ∈ V(G)) :
+--     G ≤s G.addEdge e x y := by
+--   nth_rw 1 [← addEdge_deleteEdge he hx hy]
+--   exact edgeDelete_isSpanningSubgraph
+
+-- lemma IsLink.deleteEdge_addEdge (h : G.IsLink e x y) : (G ＼ {e}).addEdge e x y = G :=
+--   ext_of_le_le (addEdge_le (by simp) h) le_rfl (by simp [pair_subset_iff, h.left_mem, h.right_mem])
+--     <| by simp [h.edge_mem]
